<?xml version="1.0" encoding="UTF-8" standalone="yes"?>
<processDataSet xmlns:m="http://lca.jrc.it/ILCD/LCIAMethod" xmlns:common="http://lca.jrc.it/ILCD/Common" xmlns:s="http://lca.jrc.it/ILCD/Source" xmlns:c="http://lca.jrc.it/ILCD/Contact" xmlns:f="http://lca.jrc.it/ILCD/Flow" xmlns="http://lca.jrc.it/ILCD/Process" xmlns:fp="http://lca.jrc.it/ILCD/FlowProperty" xmlns:u="http://lca.jrc.it/ILCD/UnitGroup" xmlns:ns9="http://www.okworx.com/ILCD/Extensions/2018/Profile" version="1.1" ns9:profile="EN_15804">
    <processInformation>
        <dataSetInformation>
            <common:UUID>880bb3c3-5eb9-431c-afe6-f4ae4c465ece</common:UUID>
            <name>
                <baseName xml:lang="de">Glas - Bundesverband Flachglas e.V. - Verbundsicherheitsglas</baseName>
                <baseName xml:lang="en">Glass - Bundesverband Flachglas e.V. - Laminated safety glass</baseName>
            </name>
            <common:synonyms xml:lang="de">VSG; Kalk-Natronsilicatglas; PVB-Folie</common:synonyms>
            <common:synonyms xml:lang="en">ESG; Soda lime silicate glass; PVB-film; LSG</common:synonyms>
            <classificationInformation>
                <common:classification>
                    <common:class level="0" classId="7">Komponenten von Fenstern und Vorhangfassaden</common:class>
                    <common:class level="1" classId="7.2">Füllungen</common:class>
                    <common:class level="2" classId="7.2.01">Transparente Füllungen</common:class>
                </common:classification>
                <common:classification name="OEKOBAU.DAT">
                    <common:class level="0" classId="7">Komponenten von Fenstern und Vorhangfassaden</common:class>
                    <common:class level="1" classId="7.2">Füllungen</common:class>
                    <common:class level="2" classId="7.2.01">Transparente Füllungen</common:class>
                </common:classification>
            </classificationInformation>
            <common:generalComment xml:lang="de">Dieser Datensatz beinhaltet die Ergebnisse für die Module A1-A3 sowie die Module C1, C2, C3, C4, D gemäß EN 15804. Ein Vergleich mit anderen Produkten ist nur mit einer vergleichbaren Anwendung im Gebäude zulässig. Grundsätzlich ist eine Gegenüberstellung oder die Bewertung von EPD Daten nur möglich, wenn alle zu vergleichenden Datensätze nach EN 15804 erstellt wurden und der Gebäudekontext, bzw. die produktspezifischen Leistungsmerkmale berücksichtigt werden.</common:generalComment>
            <common:generalComment xml:lang="en">This dataset contains the results for the modules A1-A3 and the modules C1, C2, C3, C4, D according to the European Standard EN 15804 for Sustainable Construction. The comparison with other products is only permissible if the application in the building is comparable. In principle, a comparison or the evaluation of EPD data is only possible, if all compared datasets have been generated in accordance with EN 15804 and the building context or the product-specific performance characteristics are taken into account.</common:generalComment>
        </dataSetInformation>
        <quantitativeReference type="Reference flow(s)">
            <referenceToReferenceFlow>1</referenceToReferenceFlow>
        </quantitativeReference>
        <time>
            <common:referenceYear>2017</common:referenceYear>
            <common:dataSetValidUntil>2022</common:dataSetValidUntil>
            <common:timeRepresentativenessDescription xml:lang="de">jährlicher Durchschnitt</common:timeRepresentativenessDescription>
            <common:timeRepresentativenessDescription xml:lang="en">annual average</common:timeRepresentativenessDescription>
        </time>
        <geography>
            <locationOfOperationSupplyOrProduction location="RER">
                <descriptionOfRestrictions xml:lang="de">Dieser Datensatz repräsentiert die Situation der Mitgliedsfirmen des Bundesverbands Flachglas e.V., im Hinblick auf die wichtigsten Technologien und die gesetzlichen Rahmenbedingungen.</descriptionOfRestrictions>
                <descriptionOfRestrictions xml:lang="en">This data set represents the situation of the member companies of the Bundesverband Flachglas e.V., with regard to the most important technologies and the legal framework. </descriptionOfRestrictions>
            </locationOfOperationSupplyOrProduction>
        </geography>
        <technology>
            <technologyDescriptionAndIncludedProcesses xml:lang="de">Die Ökobilanzergebnisse umfassen die Lebenszyklusstadien der Herstellung der Vorprodukte bis hin zur Rohstoffgewinnung und Verarbeitungsprozesse von als Input dienenden Sekundärstoffen (z.B. Recyclingprozesse), deren Transporte zum Werk sowie die Produktion selbst, einschließlich der Bereitstellung von allen Hilfs- und Betriebsstoffen, Energie, sowie die vollständige Abfallbehandlung oder die Deponierung der Restabfälle während des Stadiums der Produktion. Die Module A1, A2 und A3 sind hier als ein aggregiertes Modul A1-A3 ausgewiesen. Falls für diesen Datensatz weitere Module berechnet wurden, sind diese separat zu finden und können für eine Betrachtung des gesamten Lebenszyklus zusammengeführt werden.</technologyDescriptionAndIncludedProcesses>
            <technologyDescriptionAndIncludedProcesses xml:lang="en">The LCA results include the life cycle stages of the pre-products manufacture to the point of the raw material extraction and processing of secondary material input (e.g. recycling processes), their transport to the manufacturer as well as the maufacturing itself, including provision of all operating supplies, energy and the complete waste treatment or the landfill of residual waste during the stage of manufacture.&#xD;
The modules A1, A2 and A3 are shown here as an aggregated module A1-A3. If further modules have been calculated for this dataset, these can be found separately and can be merged for consideration of the entire life cycle.</technologyDescriptionAndIncludedProcesses>
            <technologicalApplicability xml:lang="de">Verbundsicherheitsglas (VSG) für die Weiterverarbeitung zu Mehrscheiben-Isolierglas und Anwendungen als Glas für das Bauwesen (Verwendung in der Gebäudehülle und beim Ausbau von baulichen Anlagen/Bauwerken).</technologicalApplicability>
            <technologicalApplicability xml:lang="en">Laminated safety glass (LSG) for processing into insulating glass units and for use as glass for buildings (in the building envelope and for finishing of works / structures).</technologicalApplicability>
        </technology>
    </processInformation>
    <modellingAndValidation>
        <LCIMethodAndAllocation>
            <typeOfDataSet>EPD</typeOfDataSet>
            <referenceToLCAMethodDetails type="source data set" refObjectId="c6e986be-62a9-4f2f-b486-27aa9129eaeb" version="00.00.002">
                <common:shortDescription xml:lang="de">Produktkategorieregeln Teil A</common:shortDescription>
            </referenceToLCAMethodDetails>
            <referenceToLCAMethodDetails type="source data set" refObjectId="b4ac8997-4a8f-4877-8461-391a44b91c1e" version="00.00.001">
                <common:shortDescription xml:lang="de">Produktkategorieregeln Teil B – für Flachglas im Bauwesen</common:shortDescription>
            </referenceToLCAMethodDetails>
            <referenceToLCAMethodDetails type="source data set" refObjectId="104410c7-6ed5-441a-8735-14b8d8cc0fbd" version="00.00.009">
                <common:shortDescription xml:lang="de">EPD Flachglas, Einscheibensicherheitsglas und Verbundsicherheitsglas</common:shortDescription>
                <common:shortDescription xml:lang="en">EPD Flat glass, toughened safety glass and laminated safety glass</common:shortDescription>
            </referenceToLCAMethodDetails>
            <common:other>
                <epd:subType xmlns:epd="http://www.iai.kit.edu/EPD/2013">representative dataset</epd:subType>
            </common:other>
        </LCIMethodAndAllocation>
        <dataSourcesTreatmentAndRepresentativeness>
            <referenceToDataSource type="source data set" refObjectId="28d74cc0-db8b-4d7e-bc44-5f6d56ce0c4a" version="00.03.001" uri="http://openlca.org/ilcd/resource/sources/28d74cc0-db8b-4d7e-bc44-5f6d56ce0c4a">
                <common:shortDescription xml:lang="en">GaBi database (all versions)</common:shortDescription>
            </referenceToDataSource>
            <useAdviceForDataSet xml:lang="de">A1-A3 sowie Module C1, C2, C3, C4, D. Das Umweltprofil beinhaltet die Aufwendungen für die Lebenszyklus-Stadien cradle to gate mit Optionen (Modul A1-A3).&#xD;
&#xD;
Der Aufbau des Verbundsicherheitsglases bezieht sich auf eine Glasdicke von 6 mm.&#xD;
&#xD;
Die Muster-EPD erlangt Gültigkeit durch die Übertragung an den Hersteller durch das ift. Aktuell gültige EPDs sind der nachfolgenden Liste zu entehmen und auf www.ift-service.de/epd veröffentlicht.&#xD;
EPD-Nummer und Deklarationsinhaber:&#xD;
- M-EPD-FEV-002001, Semcoglas Holding GmbH, 26655 Westerstede&#xD;
- M-EPD-FEV-002002, Q4Glass ABJ Investors Sp. z.o.o. Sp. k., 75-209 Koszalin&#xD;
- M-EPD-FEV-002003, arcon Flachglas-Veredelung GmbH &amp; Co. KG, 91555 Feuchtwangen&#xD;
- M-EPD-FEV-002004, Pilkington Deutschland AG, 45966 Gladbeck&#xD;
- M-EPD-FEV-002005, EUROGLAS GmbH, 39340 Haldensleben&#xD;
- M-EPD-FEV-002006, Hero-Glas Veredelungs GmbH, 26906 Dersum&#xD;
- M-EPD-FEV-002007, Glas Tech S.A., 62-020 Swarzedz&#xD;
- M-EPD-FEV-002008,  Opolglass Sp. z.o.o., 45-125 Opole&#xD;
- M-EPD-FEV-002009, thermopor glas GmbH, 52399 Merzenich&#xD;
- M-EPD-FEV-002011, Scheuten Glas Nederland Base Glass Unit, 5928 LN Venlo&#xD;
- M-EPD-FEV-002012, Scheuten Glas Nederland Glass Tech Unit,5928 LN Venlo&#xD;
- M-EPD-FEV-002013, Glas Trösch GmbH, 86720 Nördlingen&#xD;
- M-EPD-FEV-002014, Flachglas Wernberg GmbH, 92533 Wernberg-Köblitz&#xD;
- M-EPD-FEV-002015, OKALUX GmbH, 97828 Marktheidenfeld-Altfeld&#xD;
- M-EPD-FEV-002016, Brakeler Thermo-Glas, GmbH, 33034 Brakel&#xD;
- M-EPD-FEV-GB-002017, Pilkington IGP Sp. O o.o, 27-600 Sandomierz&#xD;
- M-EPD-FEV-GB-002018, PRESS GLASS SA, 42-262 Poczesna&#xD;
- M-EPD-FEV-002019, Isophon glas GmbH, 34346 Hann. Münden</useAdviceForDataSet>
            <useAdviceForDataSet xml:lang="en">A1-A3 as well as modules C1, C2, C3, C4, D. The environmental profile includes the life cycle stages cradle to gate with options.&#xD;
&#xD;
The construction of the laminated safety glass refers to a glass thickness of 6 mm.&#xD;
&#xD;
The model EPD obtains validity through the transfer to the manufacturer by the ift. Currently valid EPDs are to be taken from the list below and are published on www.ift-service.de/epd.&#xD;
EPD number and declaration holder:&#xD;
- M-EPD-FEV-002001, Semcoglas Holding GmbH, 26655 Westerstede&#xD;
- M-EPD-FEV-002002, Q4Glass ABJ Investors Sp. z.o.o. Sp. k., 75-209 Koszalin&#xD;
- M-EPD-FEV-002003, arcon Flachglas-Veredelung GmbH &amp; Co. KG, 91555 Feuchtwangen&#xD;
- M-EPD-FEV-002004, Pilkington Deutschland AG, 45966 Gladbeck&#xD;
- M-EPD-FEV-002005, EUROGLAS GmbH, 39340 Haldensleben&#xD;
- M-EPD-FEV-002006, Hero-Glas Veredelungs GmbH, 26906 Dersum&#xD;
- M-EPD-FEV-002007, Glas Tech S.A., 62-020 Swarzedz&#xD;
- M-EPD-FEV-002008,  Opolglass Sp. z.o.o., 45-125 Opole&#xD;
- M-EPD-FEV-002009, thermopor glas GmbH, 52399 Merzenich&#xD;
- M-EPD-FEV-002011, Scheuten Glas Nederland Base Glass Unit, 5928 LN Venlo&#xD;
- M-EPD-FEV-002012, Scheuten Glas Nederland Glass Tech Unit,5928 LN Venlo&#xD;
- M-EPD-FEV-002013, Glas Trösch GmbH, 86720 Nördlingen&#xD;
- M-EPD-FEV-002014, Flachglas Wernberg GmbH, 92533 Wernberg-Köblitz&#xD;
- M-EPD-FEV-002015, OKALUX GmbH, 97828 Marktheidenfeld-Altfeld&#xD;
- M-EPD-FEV-002016, Brakeler Thermo-Glas GmbH, 33034 Brakel&#xD;
- M-EPD-FEV-GB-002017, Pilkington IGP Sp. O o.o, 27-600 Sandomierz&#xD;
- M-EPD-FEV-GB-002018, PRESS GLASS SA, 42-262 Poczesna&#xD;
- M-EPD-FEV-002019, Isophon glas GmbH, 34346 Hann. Münden</useAdviceForDataSet>
        </dataSourcesTreatmentAndRepresentativeness>
        <validation>
            <review type="Independent external review">
                <common:reviewDetails xml:lang="de">Die angewendete LCI Methode ist in Übereinstimmung mit ISO 14040 und 14044. Die Dokumentation enthält alle relevanten Informationen im Hinblick auf die Datenqualität und den Umfang der Anwendung der jeweiligen LCI Ergebnisse bzw. der Datensätze. Der Datensatz repräsentiert den Stand der Technik bezogen auf die funktionelle Einheit.</common:reviewDetails>
                <common:reviewDetails xml:lang="en">The LCI method applied is in compliance with ISO 14040 and 14044. The documentation includes all relevant information in view of the data quality and scope of the application of the respective LCI result or data set. The dataset represents the state-of-the-art with regard to to the functional unit.</common:reviewDetails>
                <common:referenceToNameOfReviewerAndInstitution type="contact data set" refObjectId="4ca8370d-bd95-4619-9fe3-8c74f628b623" version="00.00.001" uri="http://openlca.org/ilcd/resource/contacts/4ca8370d-bd95-4619-9fe3-8c74f628b623">
                    <common:shortDescription xml:lang="en">Patrick Wortner</common:shortDescription>
                </common:referenceToNameOfReviewerAndInstitution>
            </review>
        </validation>
        <complianceDeclarations>
            <compliance>
                <common:referenceToComplianceSystem type="source data set" refObjectId="b00f9ec0-7874-11e3-981f-0800200c9a66" version="00.02.000">
                    <common:shortDescription xml:lang="de">EN 15804</common:shortDescription>
                    <common:shortDescription xml:lang="en">EN 15804</common:shortDescription>
                </common:referenceToComplianceSystem>
            </compliance>
        </complianceDeclarations>
    </modellingAndValidation>
    <administrativeInformation>
        <dataEntryBy>
            <common:timeStamp>2020-05-20T10:22:06.005+02:00</common:timeStamp>
            <common:referenceToDataSetFormat type="source data set" refObjectId="cba73800-7874-11e3-981f-0800200c9a66" version="00.01.000">
                <common:shortDescription xml:lang="de">EPD Data Format Extension</common:shortDescription>
            </common:referenceToDataSetFormat>
            <common:referenceToDataSetFormat type="source data set" refObjectId="a97a0155-0234-4b87-b4ce-a45da52f2a40" version="03.00.000" uri="http://lca.jrc.ec.europa.eu/lcainfohub/datasets/ilcd/sources/a97a0155-0234-4b87-b4ce-a45da52f2a40.xml">
                <common:shortDescription xml:lang="en">ILCD format</common:shortDescription>
            </common:referenceToDataSetFormat>
            <common:referenceToPersonOrEntityEnteringTheData type="contact data set" refObjectId="e4e77c13-c6e7-437a-8b76-826e43bb5a95" version="00.00.001" uri="http://openlca.org/ilcd/resource/contacts/e4e77c13-c6e7-437a-8b76-826e43bb5a95">
                <common:shortDescription xml:lang="en">ift Rosenheim</common:shortDescription>
            </common:referenceToPersonOrEntityEnteringTheData>
        </dataEntryBy>
        <publicationAndOwnership>
            <common:dataSetVersion>00.03.012</common:dataSetVersion>
            <common:referenceToOwnershipOfDataSet type="contact data set" refObjectId="010ed31f-e7ae-4984-a89c-dd2b2eae4261" version="00.00.001">
                <common:shortDescription xml:lang="de">Bundesverband Flachglas e.V.</common:shortDescription>
            </common:referenceToOwnershipOfDataSet>
            <common:copyright>true</common:copyright>
        </publicationAndOwnership>
    </administrativeInformation>
    <exchanges>
        <exchange dataSetInternalID="1">
            <referenceToFlowDataSet type="flow data set" refObjectId="8dc27d3e-aec5-4436-82a1-f4f23f8b7c34" version="01.00.002">
                <common:shortDescription xml:lang="de">Glas - Bundesverband Flachglas e.V. - Verbundsicherheitsglas</common:shortDescription>
                <common:shortDescription xml:lang="en">Glass - Bundesverband Flachglas e.V. - Laminated safety glass</common:shortDescription>
            </referenceToFlowDataSet>
            <meanAmount>1.0</meanAmount>
            <resultingAmount>1.0</resultingAmount>
        </exchange>
        <exchange dataSetInternalID="2">
            <referenceToFlowDataSet type="flow data set" refObjectId="a2b32f97-3fc7-4af2-b209-525bc6426f33" version="30.00.000">
                <common:shortDescription xml:lang="en">Components for re-use (CRU)</common:shortDescription>
                <common:shortDescription xml:lang="de">Komponenten für die Wiederverwendung (CRU)</common:shortDescription>
                <common:shortDescription xml:lang="es">Componentes para su reutilización (CRU)</common:shortDescription>
            </referenceToFlowDataSet>
            <functionType>General reminder flow</functionType>
            <exchangeDirection>Output</exchangeDirection>
            <meanAmount>0.0</meanAmount>
            <common:other>
                <epd:amount xmlns:epd="http://www.iai.kit.edu/EPD/2013" epd:module="A1-A3">0.0</epd:amount>
                <epd:amount xmlns:epd="http://www.iai.kit.edu/EPD/2013" epd:module="C1">0.0</epd:amount>
                <epd:amount xmlns:epd="http://www.iai.kit.edu/EPD/2013" epd:module="C2">0.0</epd:amount>
                <epd:amount xmlns:epd="http://www.iai.kit.edu/EPD/2013" epd:module="C3">0.0</epd:amount>
                <epd:amount xmlns:epd="http://www.iai.kit.edu/EPD/2013" epd:module="C4">0.0</epd:amount>
                <epd:amount xmlns:epd="http://www.iai.kit.edu/EPD/2013" epd:module="D"/>
                <epd:referenceToUnitGroupDataSet xmlns:epd="http://www.iai.kit.edu/EPD/2013" refObjectId="ad38d542-3fe9-439d-9b95-2f5f7752acaf" type="unit group data set" uri="../unitgroups/ad38d542-3fe9-439d-9b95-2f5f7752acaf">
                    <common:shortDescription>kg</common:shortDescription>
                </epd:referenceToUnitGroupDataSet>
            </common:other>
        </exchange>
        <exchange dataSetInternalID="3">
            <referenceToFlowDataSet type="flow data set" refObjectId="4da0c987-2b76-40d6-9e9e-82a017aaaf29" version="30.00.000">
                <common:shortDescription xml:lang="en">Exported electrical energy (EEE)</common:shortDescription>
                <common:shortDescription xml:lang="de">Exportierte elektrische Energie (EEE)</common:shortDescription>
                <common:shortDescription xml:lang="es">Energía exportada electrica (EEE)</common:shortDescription>
            </referenceToFlowDataSet>
            <functionType>General reminder flow</functionType>
            <exchangeDirection>Output</exchangeDirection>
            <meanAmount>0.0</meanAmount>
            <common:other>
                <epd:amount xmlns:epd="http://www.iai.kit.edu/EPD/2013" epd:module="A1-A3">1.71033</epd:amount>
                <epd:amount xmlns:epd="http://www.iai.kit.edu/EPD/2013" epd:module="C1">0.0</epd:amount>
                <epd:amount xmlns:epd="http://www.iai.kit.edu/EPD/2013" epd:module="C2">0.0</epd:amount>
                <epd:amount xmlns:epd="http://www.iai.kit.edu/EPD/2013" epd:module="C3">0.0</epd:amount>
                <epd:amount xmlns:epd="http://www.iai.kit.edu/EPD/2013" epd:module="C4">0.0</epd:amount>
                <epd:amount xmlns:epd="http://www.iai.kit.edu/EPD/2013" epd:module="D"/>
                <epd:referenceToUnitGroupDataSet xmlns:epd="http://www.iai.kit.edu/EPD/2013" refObjectId="93a60a57-a3c8-11da-a746-0800200c9a66" type="unit group data set" uri="../unitgroups/93a60a57-a3c8-11da-a746-0800200c9a66">
                    <common:shortDescription>MJ</common:shortDescription>
                </epd:referenceToUnitGroupDataSet>
            </common:other>
        </exchange>
        <exchange dataSetInternalID="4">
            <referenceToFlowDataSet type="flow data set" refObjectId="98daf38a-7a79-46d3-9a37-2b7bd0955810" version="30.00.000">
                <common:shortDescription xml:lang="en">Exported thermal energy (EET)</common:shortDescription>
                <common:shortDescription xml:lang="de">Exportierte thermische Energie (EET)</common:shortDescription>
                <common:shortDescription xml:lang="es">Energía exportada termal (EET)</common:shortDescription>
            </referenceToFlowDataSet>
            <functionType>General reminder flow</functionType>
            <exchangeDirection>Output</exchangeDirection>
            <meanAmount>0.0</meanAmount>
            <common:other>
                <epd:amount xmlns:epd="http://www.iai.kit.edu/EPD/2013" epd:module="A1-A3">3.2084339999999996</epd:amount>
                <epd:amount xmlns:epd="http://www.iai.kit.edu/EPD/2013" epd:module="C1">0.0</epd:amount>
                <epd:amount xmlns:epd="http://www.iai.kit.edu/EPD/2013" epd:module="C2">0.0</epd:amount>
                <epd:amount xmlns:epd="http://www.iai.kit.edu/EPD/2013" epd:module="C3">0.0</epd:amount>
                <epd:amount xmlns:epd="http://www.iai.kit.edu/EPD/2013" epd:module="C4">0.0</epd:amount>
                <epd:amount xmlns:epd="http://www.iai.kit.edu/EPD/2013" epd:module="D"/>
                <epd:referenceToUnitGroupDataSet xmlns:epd="http://www.iai.kit.edu/EPD/2013" refObjectId="93a60a57-a3c8-11da-a746-0800200c9a66" type="unit group data set" uri="../unitgroups/93a60a57-a3c8-11da-a746-0800200c9a66">
                    <common:shortDescription>MJ</common:shortDescription>
                </epd:referenceToUnitGroupDataSet>
            </common:other>
        </exchange>
        <exchange dataSetInternalID="5">
            <referenceToFlowDataSet type="flow data set" refObjectId="430f9e0f-59b2-46a0-8e0d-55e0e84948fc" version="30.00.000">
                <common:shortDescription xml:lang="en">Hazardous waste disposed (HWD)</common:shortDescription>
                <common:shortDescription xml:lang="de">Gefährlicher Abfall zur Deponie (HWD)</common:shortDescription>
                <common:shortDescription xml:lang="es">Residuos peligrosos eliminados (HWD)</common:shortDescription>
            </referenceToFlowDataSet>
            <functionType>General reminder flow</functionType>
            <exchangeDirection>Output</exchangeDirection>
            <meanAmount>0.0</meanAmount>
            <common:other>
                <epd:amount xmlns:epd="http://www.iai.kit.edu/EPD/2013" epd:module="A1-A3">8.53236E-7</epd:amount>
                <epd:amount xmlns:epd="http://www.iai.kit.edu/EPD/2013" epd:module="C1">1.511124E-9</epd:amount>
                <epd:amount xmlns:epd="http://www.iai.kit.edu/EPD/2013" epd:module="C2">4.6141019999999996E-8</epd:amount>
                <epd:amount xmlns:epd="http://www.iai.kit.edu/EPD/2013" epd:module="C3">2.2017119999999996E-9</epd:amount>
                <epd:amount xmlns:epd="http://www.iai.kit.edu/EPD/2013" epd:module="C4">3.98409E-8</epd:amount>
                <epd:amount xmlns:epd="http://www.iai.kit.edu/EPD/2013" epd:module="D">-3.536232E-8</epd:amount>
                <epd:referenceToUnitGroupDataSet xmlns:epd="http://www.iai.kit.edu/EPD/2013" refObjectId="ad38d542-3fe9-439d-9b95-2f5f7752acaf" type="unit group data set" uri="../unitgroups/ad38d542-3fe9-439d-9b95-2f5f7752acaf">
                    <common:shortDescription>kg</common:shortDescription>
                </epd:referenceToUnitGroupDataSet>
            </common:other>
        </exchange>
        <exchange dataSetInternalID="6">
            <referenceToFlowDataSet type="flow data set" refObjectId="59a9181c-3aaf-46ee-8b13-2b3723b6e447" version="30.00.000">
                <common:shortDescription xml:lang="en">Materials for energy recovery (MER)</common:shortDescription>
                <common:shortDescription xml:lang="de">Stoffe für die Energierückgewinnung (MER)</common:shortDescription>
                <common:shortDescription xml:lang="es">Materiales para valorización energética (recuperación de energía) (MER)</common:shortDescription>
            </referenceToFlowDataSet>
            <functionType>General reminder flow</functionType>
            <exchangeDirection>Output</exchangeDirection>
            <meanAmount>0.0</meanAmount>
            <common:other>
                <epd:amount xmlns:epd="http://www.iai.kit.edu/EPD/2013" epd:module="A1-A3">0.0</epd:amount>
                <epd:amount xmlns:epd="http://www.iai.kit.edu/EPD/2013" epd:module="C1">0.0</epd:amount>
                <epd:amount xmlns:epd="http://www.iai.kit.edu/EPD/2013" epd:module="C2">0.0</epd:amount>
                <epd:amount xmlns:epd="http://www.iai.kit.edu/EPD/2013" epd:module="C3">0.0</epd:amount>
                <epd:amount xmlns:epd="http://www.iai.kit.edu/EPD/2013" epd:module="C4">0.0</epd:amount>
                <epd:amount xmlns:epd="http://www.iai.kit.edu/EPD/2013" epd:module="D"/>
                <epd:referenceToUnitGroupDataSet xmlns:epd="http://www.iai.kit.edu/EPD/2013" refObjectId="ad38d542-3fe9-439d-9b95-2f5f7752acaf" type="unit group data set" uri="../unitgroups/ad38d542-3fe9-439d-9b95-2f5f7752acaf">
                    <common:shortDescription>kg</common:shortDescription>
                </epd:referenceToUnitGroupDataSet>
            </common:other>
        </exchange>
        <exchange dataSetInternalID="7">
            <referenceToFlowDataSet type="flow data set" refObjectId="d7fe48a5-4103-49c8-9aae-b0b5dfdbd6ae" version="30.00.000">
                <common:shortDescription xml:lang="en">Materials for recycling (MFR)</common:shortDescription>
                <common:shortDescription xml:lang="de">Stoffe zum Recycling (MFR)</common:shortDescription>
                <common:shortDescription xml:lang="es">Materiales para el reciclaje (MFR)</common:shortDescription>
            </referenceToFlowDataSet>
            <functionType>General reminder flow</functionType>
            <exchangeDirection>Output</exchangeDirection>
            <meanAmount>0.0</meanAmount>
            <common:other>
                <epd:amount xmlns:epd="http://www.iai.kit.edu/EPD/2013" epd:module="A1-A3">2.25678</epd:amount>
                <epd:amount xmlns:epd="http://www.iai.kit.edu/EPD/2013" epd:module="C1">0.0</epd:amount>
                <epd:amount xmlns:epd="http://www.iai.kit.edu/EPD/2013" epd:module="C2">0.0</epd:amount>
                <epd:amount xmlns:epd="http://www.iai.kit.edu/EPD/2013" epd:module="C3">4.45842</epd:amount>
                <epd:amount xmlns:epd="http://www.iai.kit.edu/EPD/2013" epd:module="C4">0.0</epd:amount>
                <epd:amount xmlns:epd="http://www.iai.kit.edu/EPD/2013" epd:module="D"/>
                <epd:referenceToUnitGroupDataSet xmlns:epd="http://www.iai.kit.edu/EPD/2013" refObjectId="ad38d542-3fe9-439d-9b95-2f5f7752acaf" type="unit group data set" uri="../unitgroups/ad38d542-3fe9-439d-9b95-2f5f7752acaf">
                    <common:shortDescription>kg</common:shortDescription>
                </epd:referenceToUnitGroupDataSet>
            </common:other>
        </exchange>
        <exchange dataSetInternalID="8">
            <referenceToFlowDataSet type="flow data set" refObjectId="3cf952c8-f3a4-461d-8c96-96456ca62246" version="30.00.000">
                <common:shortDescription xml:lang="en">Use of net fresh water (FW)</common:shortDescription>
                <common:shortDescription xml:lang="de">Einsatz von Süßwasserressourcen (FW)</common:shortDescription>
                <common:shortDescription xml:lang="es">Uso neto de recursos de agua dulce (FW)</common:shortDescription>
            </referenceToFlowDataSet>
            <functionType>General reminder flow</functionType>
            <exchangeDirection>Input</exchangeDirection>
            <meanAmount>0.0</meanAmount>
            <common:other>
                <epd:amount xmlns:epd="http://www.iai.kit.edu/EPD/2013" epd:module="A1-A3">0.3100326</epd:amount>
                <epd:amount xmlns:epd="http://www.iai.kit.edu/EPD/2013" epd:module="C1">0.0016493220000000002</epd:amount>
                <epd:amount xmlns:epd="http://www.iai.kit.edu/EPD/2013" epd:module="C2">8.11092E-5</epd:amount>
                <epd:amount xmlns:epd="http://www.iai.kit.edu/EPD/2013" epd:module="C3">0.0024030600000000003</epd:amount>
                <epd:amount xmlns:epd="http://www.iai.kit.edu/EPD/2013" epd:module="C4">4.4234280000000003E-4</epd:amount>
                <epd:amount xmlns:epd="http://www.iai.kit.edu/EPD/2013" epd:module="D">-0.004872042</epd:amount>
                <epd:referenceToUnitGroupDataSet xmlns:epd="http://www.iai.kit.edu/EPD/2013" refObjectId="cd950537-0a98-4044-9ba7-9f9a68d0a504" type="unit group data set" uri="../unitgroups/cd950537-0a98-4044-9ba7-9f9a68d0a504">
                    <common:shortDescription>m3</common:shortDescription>
                </epd:referenceToUnitGroupDataSet>
            </common:other>
        </exchange>
        <exchange dataSetInternalID="9">
            <referenceToFlowDataSet type="flow data set" refObjectId="b29ef66b-e286-4afa-949f-62f1a7b4d7fa" version="30.00.000">
                <common:shortDescription xml:lang="en">Non hazardous waste dispose (NHWD)</common:shortDescription>
                <common:shortDescription xml:lang="de">Entsorgter nicht gefährlicher Abfall (NHWD)</common:shortDescription>
                <common:shortDescription xml:lang="es">Residuos no peligrosos eliminados (NHWD)</common:shortDescription>
            </referenceToFlowDataSet>
            <functionType>General reminder flow</functionType>
            <exchangeDirection>Output</exchangeDirection>
            <meanAmount>0.0</meanAmount>
            <common:other>
                <epd:amount xmlns:epd="http://www.iai.kit.edu/EPD/2013" epd:module="A1-A3">19.378619999999998</epd:amount>
                <epd:amount xmlns:epd="http://www.iai.kit.edu/EPD/2013" epd:module="C1">0.002269362</epd:amount>
                <epd:amount xmlns:epd="http://www.iai.kit.edu/EPD/2013" epd:module="C2">6.68484E-5</epd:amount>
                <epd:amount xmlns:epd="http://www.iai.kit.edu/EPD/2013" epd:module="C3">0.0033064619999999996</epd:amount>
                <epd:amount xmlns:epd="http://www.iai.kit.edu/EPD/2013" epd:module="C4">10.86078</epd:amount>
                <epd:amount xmlns:epd="http://www.iai.kit.edu/EPD/2013" epd:module="D">-0.3111816</epd:amount>
                <epd:referenceToUnitGroupDataSet xmlns:epd="http://www.iai.kit.edu/EPD/2013" refObjectId="ad38d542-3fe9-439d-9b95-2f5f7752acaf" type="unit group data set" uri="../unitgroups/ad38d542-3fe9-439d-9b95-2f5f7752acaf">
                    <common:shortDescription>kg</common:shortDescription>
                </epd:referenceToUnitGroupDataSet>
            </common:other>
        </exchange>
        <exchange dataSetInternalID="10">
            <referenceToFlowDataSet type="flow data set" refObjectId="ac857178-2b45-46ec-892a-a9a4332f0372" version="30.00.000">
                <common:shortDescription xml:lang="en">Use of non renewable primary energy (PENRE)</common:shortDescription>
                <common:shortDescription xml:lang="de">Nicht-erneuerbare Primärenergie als Energieträger (PENRE)</common:shortDescription>
                <common:shortDescription xml:lang="es">Uso de energía primaria no renovable, excluyendo los recursos de energía primaria no renovable utilizada como materia prima (PENRE)</common:shortDescription>
            </referenceToFlowDataSet>
            <functionType>General reminder flow</functionType>
            <exchangeDirection>Input</exchangeDirection>
            <meanAmount>0.0</meanAmount>
            <common:other>
                <epd:amount xmlns:epd="http://www.iai.kit.edu/EPD/2013" epd:module="A1-A3">838.602</epd:amount>
                <epd:amount xmlns:epd="http://www.iai.kit.edu/EPD/2013" epd:module="C1">3.2216760000000004</epd:amount>
                <epd:amount xmlns:epd="http://www.iai.kit.edu/EPD/2013" epd:module="C2">0.798</epd:amount>
                <epd:amount xmlns:epd="http://www.iai.kit.edu/EPD/2013" epd:module="C3">4.69398</epd:amount>
                <epd:amount xmlns:epd="http://www.iai.kit.edu/EPD/2013" epd:module="C4">10.955412</epd:amount>
                <epd:amount xmlns:epd="http://www.iai.kit.edu/EPD/2013" epd:module="D">-33.832440000000005</epd:amount>
                <epd:referenceToUnitGroupDataSet xmlns:epd="http://www.iai.kit.edu/EPD/2013" refObjectId="93a60a57-a3c8-11da-a746-0800200c9a66" type="unit group data set" uri="../unitgroups/93a60a57-a3c8-11da-a746-0800200c9a66">
                    <common:shortDescription>MJ</common:shortDescription>
                </epd:referenceToUnitGroupDataSet>
            </common:other>
        </exchange>
        <exchange dataSetInternalID="11">
            <referenceToFlowDataSet type="flow data set" refObjectId="1421caa0-679d-4bf4-b282-0eb850ccae27" version="30.00.000">
                <common:shortDescription xml:lang="en">Use of non renewable primary energy resources used as raw materials (PENRM)</common:shortDescription>
                <common:shortDescription xml:lang="de">Nicht-erneuerbare Primärenergie zur stofflichen Nutzung (PENRM)</common:shortDescription>
                <common:shortDescription xml:lang="es">Uso de la energía primaria no renovable utilizada como materia prima (PENRM)</common:shortDescription>
            </referenceToFlowDataSet>
            <functionType>General reminder flow</functionType>
            <exchangeDirection>Input</exchangeDirection>
            <meanAmount>0.0</meanAmount>
            <common:other>
                <epd:amount xmlns:epd="http://www.iai.kit.edu/EPD/2013" epd:module="A1-A3">8.64</epd:amount>
                <epd:amount xmlns:epd="http://www.iai.kit.edu/EPD/2013" epd:module="C1">0.0</epd:amount>
                <epd:amount xmlns:epd="http://www.iai.kit.edu/EPD/2013" epd:module="C2">0.0</epd:amount>
                <epd:amount xmlns:epd="http://www.iai.kit.edu/EPD/2013" epd:module="C3">0.0</epd:amount>
                <epd:amount xmlns:epd="http://www.iai.kit.edu/EPD/2013" epd:module="C4">-8.64</epd:amount>
                <epd:amount xmlns:epd="http://www.iai.kit.edu/EPD/2013" epd:module="D">0.0</epd:amount>
                <epd:referenceToUnitGroupDataSet xmlns:epd="http://www.iai.kit.edu/EPD/2013" refObjectId="93a60a57-a3c8-11da-a746-0800200c9a66" type="unit group data set" uri="../unitgroups/93a60a57-a3c8-11da-a746-0800200c9a66">
                    <common:shortDescription>MJ</common:shortDescription>
                </epd:referenceToUnitGroupDataSet>
            </common:other>
        </exchange>
        <exchange dataSetInternalID="12">
            <referenceToFlowDataSet type="flow data set" refObjectId="89def144-d39a-4287-b86f-efde453ddcb2" version="30.00.000">
                <common:shortDescription xml:lang="en">Use of non renewable secondary fuels (NRSF)</common:shortDescription>
                <common:shortDescription xml:lang="de">Nicht erneuerbare Sekundärbrennstoffe (NRSF)</common:shortDescription>
                <common:shortDescription xml:lang="es">Uso de combustibles secundarios no renovables (NRSF)</common:shortDescription>
            </referenceToFlowDataSet>
            <functionType>General reminder flow</functionType>
            <exchangeDirection>Input</exchangeDirection>
            <meanAmount>0.0</meanAmount>
            <common:other>
                <epd:amount xmlns:epd="http://www.iai.kit.edu/EPD/2013" epd:module="A1-A3">2.0020500000000002E-19</epd:amount>
                <epd:amount xmlns:epd="http://www.iai.kit.edu/EPD/2013" epd:module="C1">4.787238E-30</epd:amount>
                <epd:amount xmlns:epd="http://www.iai.kit.edu/EPD/2013" epd:module="C2">6.538260000000001E-29</epd:amount>
                <epd:amount xmlns:epd="http://www.iai.kit.edu/EPD/2013" epd:module="C3">6.975E-30</epd:amount>
                <epd:amount xmlns:epd="http://www.iai.kit.edu/EPD/2013" epd:module="C4">4.1211960000000003E-22</epd:amount>
                <epd:amount xmlns:epd="http://www.iai.kit.edu/EPD/2013" epd:module="D">-1.7036039999999998E-20</epd:amount>
                <epd:referenceToUnitGroupDataSet xmlns:epd="http://www.iai.kit.edu/EPD/2013" refObjectId="93a60a57-a3c8-11da-a746-0800200c9a66" type="unit group data set" uri="../unitgroups/93a60a57-a3c8-11da-a746-0800200c9a66">
                    <common:shortDescription>MJ</common:shortDescription>
                </epd:referenceToUnitGroupDataSet>
            </common:other>
        </exchange>
        <exchange dataSetInternalID="13">
            <referenceToFlowDataSet type="flow data set" refObjectId="3449546e-52ad-4b39-b809-9fb77cea8ff6" version="30.00.000">
                <common:shortDescription xml:lang="en">Radioactive waste disposed (RWD)</common:shortDescription>
                <common:shortDescription xml:lang="de">Entsorgter radioaktiver Abfall (RWD)</common:shortDescription>
                <common:shortDescription xml:lang="es">Residuos radiactivos eliminados (RWD)</common:shortDescription>
            </referenceToFlowDataSet>
            <functionType>General reminder flow</functionType>
            <exchangeDirection>Output</exchangeDirection>
            <meanAmount>0.0</meanAmount>
            <common:other>
                <epd:amount xmlns:epd="http://www.iai.kit.edu/EPD/2013" epd:module="A1-A3">0.0808236</epd:amount>
                <epd:amount xmlns:epd="http://www.iai.kit.edu/EPD/2013" epd:module="C1">5.334960000000001E-4</epd:amount>
                <epd:amount xmlns:epd="http://www.iai.kit.edu/EPD/2013" epd:module="C2">1.092126E-6</epd:amount>
                <epd:amount xmlns:epd="http://www.iai.kit.edu/EPD/2013" epd:module="C3">7.77306E-4</epd:amount>
                <epd:amount xmlns:epd="http://www.iai.kit.edu/EPD/2013" epd:module="C4">3.355206E-5</epd:amount>
                <epd:amount xmlns:epd="http://www.iai.kit.edu/EPD/2013" epd:module="D">-9.435E-4</epd:amount>
                <epd:referenceToUnitGroupDataSet xmlns:epd="http://www.iai.kit.edu/EPD/2013" refObjectId="ad38d542-3fe9-439d-9b95-2f5f7752acaf" type="unit group data set" uri="../unitgroups/ad38d542-3fe9-439d-9b95-2f5f7752acaf">
                    <common:shortDescription>kg</common:shortDescription>
                </epd:referenceToUnitGroupDataSet>
            </common:other>
        </exchange>
        <exchange dataSetInternalID="14">
            <referenceToFlowDataSet type="flow data set" refObjectId="20f32be5-0398-4288-9b6d-accddd195317" version="30.00.000">
                <common:shortDescription xml:lang="en">Use of renewable primary energy (PERE)</common:shortDescription>
                <common:shortDescription xml:lang="de">Erneuerbare Primärenergie als Energieträger (PERE)</common:shortDescription>
                <common:shortDescription xml:lang="es">Uso de energía primaria renovable excluyendo los recursos de energía primaria renovable utilizada como materia prima (PERE)</common:shortDescription>
            </referenceToFlowDataSet>
            <functionType>General reminder flow</functionType>
            <exchangeDirection>Input</exchangeDirection>
            <meanAmount>0.0</meanAmount>
            <common:other>
                <epd:amount xmlns:epd="http://www.iai.kit.edu/EPD/2013" epd:module="A1-A3">184.40879999999999</epd:amount>
                <epd:amount xmlns:epd="http://www.iai.kit.edu/EPD/2013" epd:module="C1">1.210386</epd:amount>
                <epd:amount xmlns:epd="http://www.iai.kit.edu/EPD/2013" epd:module="C2">0.04401426</epd:amount>
                <epd:amount xmlns:epd="http://www.iai.kit.edu/EPD/2013" epd:module="C3">1.763532</epd:amount>
                <epd:amount xmlns:epd="http://www.iai.kit.edu/EPD/2013" epd:module="C4">0.2867364</epd:amount>
                <epd:amount xmlns:epd="http://www.iai.kit.edu/EPD/2013" epd:module="D">-2.26626</epd:amount>
                <epd:referenceToUnitGroupDataSet xmlns:epd="http://www.iai.kit.edu/EPD/2013" refObjectId="93a60a57-a3c8-11da-a746-0800200c9a66" type="unit group data set" uri="../unitgroups/93a60a57-a3c8-11da-a746-0800200c9a66">
                    <common:shortDescription>MJ</common:shortDescription>
                </epd:referenceToUnitGroupDataSet>
            </common:other>
        </exchange>
        <exchange dataSetInternalID="15">
            <referenceToFlowDataSet type="flow data set" refObjectId="fb3ec0de-548d-4508-aea5-00b73bf6f702" version="30.00.000">
                <common:shortDescription xml:lang="en">Use of renewable primary energy resources used as raw materials (PERM)</common:shortDescription>
                <common:shortDescription xml:lang="de">Erneuerbare Primärenergie zur stofflichen Nutzung (PERM)</common:shortDescription>
                <common:shortDescription xml:lang="es">Uso de energía primaria renovable utilizada como materia prima (PERM)</common:shortDescription>
            </referenceToFlowDataSet>
            <functionType>General reminder flow</functionType>
            <exchangeDirection>Input</exchangeDirection>
            <meanAmount>0.0</meanAmount>
            <common:other>
                <epd:amount xmlns:epd="http://www.iai.kit.edu/EPD/2013" epd:module="A1-A3">0.0</epd:amount>
                <epd:amount xmlns:epd="http://www.iai.kit.edu/EPD/2013" epd:module="C1">0.0</epd:amount>
                <epd:amount xmlns:epd="http://www.iai.kit.edu/EPD/2013" epd:module="C2">0.0</epd:amount>
                <epd:amount xmlns:epd="http://www.iai.kit.edu/EPD/2013" epd:module="C3">0.0</epd:amount>
                <epd:amount xmlns:epd="http://www.iai.kit.edu/EPD/2013" epd:module="C4">0.0</epd:amount>
                <epd:amount xmlns:epd="http://www.iai.kit.edu/EPD/2013" epd:module="D">0.0</epd:amount>
                <epd:referenceToUnitGroupDataSet xmlns:epd="http://www.iai.kit.edu/EPD/2013" refObjectId="93a60a57-a3c8-11da-a746-0800200c9a66" type="unit group data set" uri="../unitgroups/93a60a57-a3c8-11da-a746-0800200c9a66">
                    <common:shortDescription>MJ</common:shortDescription>
                </epd:referenceToUnitGroupDataSet>
            </common:other>
        </exchange>
        <exchange dataSetInternalID="16">
            <referenceToFlowDataSet type="flow data set" refObjectId="64333088-a55f-4aa2-9a31-c10b07816787" version="30.00.000">
                <common:shortDescription xml:lang="en">Use of renewable secondary fuels (RSF)</common:shortDescription>
                <common:shortDescription xml:lang="de">Erneuerbare Sekundärbrennstoffe (RSF)</common:shortDescription>
                <common:shortDescription xml:lang="es">Uso de combustibles secundarios renovables (RSF)</common:shortDescription>
            </referenceToFlowDataSet>
            <functionType>General reminder flow</functionType>
            <exchangeDirection>Input</exchangeDirection>
            <meanAmount>0.0</meanAmount>
            <common:other>
                <epd:amount xmlns:epd="http://www.iai.kit.edu/EPD/2013" epd:module="A1-A3">1.70442E-20</epd:amount>
                <epd:amount xmlns:epd="http://www.iai.kit.edu/EPD/2013" epd:module="C1">0.0</epd:amount>
                <epd:amount xmlns:epd="http://www.iai.kit.edu/EPD/2013" epd:module="C2">4.3090079999999995E-30</epd:amount>
                <epd:amount xmlns:epd="http://www.iai.kit.edu/EPD/2013" epd:module="C3">0.0</epd:amount>
                <epd:amount xmlns:epd="http://www.iai.kit.edu/EPD/2013" epd:module="C4">3.50853E-23</epd:amount>
                <epd:amount xmlns:epd="http://www.iai.kit.edu/EPD/2013" epd:module="D">-1.450344E-21</epd:amount>
                <epd:referenceToUnitGroupDataSet xmlns:epd="http://www.iai.kit.edu/EPD/2013" refObjectId="93a60a57-a3c8-11da-a746-0800200c9a66" type="unit group data set" uri="../unitgroups/93a60a57-a3c8-11da-a746-0800200c9a66">
                    <common:shortDescription>MJ</common:shortDescription>
                </epd:referenceToUnitGroupDataSet>
            </common:other>
        </exchange>
        <exchange dataSetInternalID="17">
            <referenceToFlowDataSet type="flow data set" refObjectId="c6a1f35f-2d09-4f54-8dfb-97e502e1ce92" version="30.00.000">
                <common:shortDescription xml:lang="en">Use of secondary material (SM)</common:shortDescription>
                <common:shortDescription xml:lang="de">Einsatz von Sekundärstoffen (SM)</common:shortDescription>
                <common:shortDescription xml:lang="es">Uso de materiales secundarios (SM)</common:shortDescription>
            </referenceToFlowDataSet>
            <functionType>General reminder flow</functionType>
            <exchangeDirection>Input</exchangeDirection>
            <meanAmount>0.0</meanAmount>
            <common:other>
                <epd:amount xmlns:epd="http://www.iai.kit.edu/EPD/2013" epd:module="A1-A3">0.7334700000000001</epd:amount>
                <epd:amount xmlns:epd="http://www.iai.kit.edu/EPD/2013" epd:module="C1">0.0</epd:amount>
                <epd:amount xmlns:epd="http://www.iai.kit.edu/EPD/2013" epd:module="C2">0.0</epd:amount>
                <epd:amount xmlns:epd="http://www.iai.kit.edu/EPD/2013" epd:module="C3">0.0</epd:amount>
                <epd:amount xmlns:epd="http://www.iai.kit.edu/EPD/2013" epd:module="C4">0.0</epd:amount>
                <epd:amount xmlns:epd="http://www.iai.kit.edu/EPD/2013" epd:module="D">0.0</epd:amount>
                <epd:referenceToUnitGroupDataSet xmlns:epd="http://www.iai.kit.edu/EPD/2013" refObjectId="ad38d542-3fe9-439d-9b95-2f5f7752acaf" type="unit group data set" uri="../unitgroups/ad38d542-3fe9-439d-9b95-2f5f7752acaf">
                    <common:shortDescription>kg</common:shortDescription>
                </epd:referenceToUnitGroupDataSet>
            </common:other>
        </exchange>
        <exchange dataSetInternalID="18">
            <referenceToFlowDataSet type="flow data set" refObjectId="06159210-646b-4c8d-8583-da9b3b95a6c1" version="30.00.000">
                <common:shortDescription xml:lang="en">Total use of non renewable primary energy resource (PENRT)</common:shortDescription>
                <common:shortDescription xml:lang="de">Total nicht erneuerbare Primärenergie (PENRT)</common:shortDescription>
                <common:shortDescription xml:lang="es">Uso total de la energía primaria no renovable (energía primaria y recursos de energía primaria renovable utilizada como materia prima) (PENRT)</common:shortDescription>
            </referenceToFlowDataSet>
            <functionType>General reminder flow</functionType>
            <exchangeDirection>Input</exchangeDirection>
            <meanAmount>0.0</meanAmount>
            <common:other>
                <epd:amount xmlns:epd="http://www.iai.kit.edu/EPD/2013" epd:module="A1-A3">847.242</epd:amount>
                <epd:amount xmlns:epd="http://www.iai.kit.edu/EPD/2013" epd:module="C1">3.2216760000000004</epd:amount>
                <epd:amount xmlns:epd="http://www.iai.kit.edu/EPD/2013" epd:module="C2">0.798</epd:amount>
                <epd:amount xmlns:epd="http://www.iai.kit.edu/EPD/2013" epd:module="C3">4.69398</epd:amount>
                <epd:amount xmlns:epd="http://www.iai.kit.edu/EPD/2013" epd:module="C4">2.3154120000000002</epd:amount>
                <epd:amount xmlns:epd="http://www.iai.kit.edu/EPD/2013" epd:module="D">-33.832440000000005</epd:amount>
                <epd:referenceToUnitGroupDataSet xmlns:epd="http://www.iai.kit.edu/EPD/2013" refObjectId="93a60a57-a3c8-11da-a746-0800200c9a66" type="unit group data set" uri="../unitgroups/93a60a57-a3c8-11da-a746-0800200c9a66">
                    <common:shortDescription>MJ</common:shortDescription>
                </epd:referenceToUnitGroupDataSet>
            </common:other>
        </exchange>
        <exchange dataSetInternalID="19">
            <referenceToFlowDataSet type="flow data set" refObjectId="53f97275-fa8a-4cdd-9024-65936002acd0" version="30.00.000">
                <common:shortDescription xml:lang="en">Total use of renewable primary energy resources (PERT)</common:shortDescription>
                <common:shortDescription xml:lang="de">Total erneuerbare Primärenergie (PERT)</common:shortDescription>
                <common:shortDescription xml:lang="es">Uso total de la energía primaria renovable (energía primaria y recursos de energía primaria renovable utilizada como materia prima) (PERT)</common:shortDescription>
            </referenceToFlowDataSet>
            <functionType>General reminder flow</functionType>
            <exchangeDirection>Input</exchangeDirection>
            <meanAmount>0.0</meanAmount>
            <common:other>
                <epd:amount xmlns:epd="http://www.iai.kit.edu/EPD/2013" epd:module="A1-A3">184.40879999999999</epd:amount>
                <epd:amount xmlns:epd="http://www.iai.kit.edu/EPD/2013" epd:module="C1">1.210386</epd:amount>
                <epd:amount xmlns:epd="http://www.iai.kit.edu/EPD/2013" epd:module="C2">0.04401426</epd:amount>
                <epd:amount xmlns:epd="http://www.iai.kit.edu/EPD/2013" epd:module="C3">1.763532</epd:amount>
                <epd:amount xmlns:epd="http://www.iai.kit.edu/EPD/2013" epd:module="C4">0.2867364</epd:amount>
                <epd:amount xmlns:epd="http://www.iai.kit.edu/EPD/2013" epd:module="D">-2.26626</epd:amount>
                <epd:referenceToUnitGroupDataSet xmlns:epd="http://www.iai.kit.edu/EPD/2013" refObjectId="93a60a57-a3c8-11da-a746-0800200c9a66" type="unit group data set" uri="../unitgroups/93a60a57-a3c8-11da-a746-0800200c9a66">
                    <common:shortDescription>MJ</common:shortDescription>
                </epd:referenceToUnitGroupDataSet>
            </common:other>
        </exchange>
    </exchanges>
    <LCIAResults>
        <LCIAResult>
            <referenceToLCIAMethodDataSet type="LCIA method data set" refObjectId="f7c73bb9-ab1a-4249-9c6d-379a0de6f67e" version="00.01.000">
                <common:shortDescription xml:lang="en">Abiotic depletion potential for non fossil resources (ADPE)</common:shortDescription>
                <common:shortDescription xml:lang="de">Potenzial für den abiotischen Abbau nicht fossiler Ressourcen (ADPE)</common:shortDescription>
                <common:shortDescription xml:lang="es">Potencial de agotamiento de recursos abióticos para recursos no fósiles (ADPE)</common:shortDescription>
            </referenceToLCIAMethodDataSet>
            <meanAmount>0.0</meanAmount>
            <common:other>
                <epd:amount xmlns:epd="http://www.iai.kit.edu/EPD/2013" epd:module="A1-A3">3.6501359999999996E-4</epd:amount>
                <epd:amount xmlns:epd="http://www.iai.kit.edu/EPD/2013" epd:module="C1">9.37056E-8</epd:amount>
                <epd:amount xmlns:epd="http://www.iai.kit.edu/EPD/2013" epd:module="C2">4.79757E-9</epd:amount>
                <epd:amount xmlns:epd="http://www.iai.kit.edu/EPD/2013" epd:module="C3">1.3652939999999999E-7</epd:amount>
                <epd:amount xmlns:epd="http://www.iai.kit.edu/EPD/2013" epd:module="C4">6.62778E-8</epd:amount>
                <epd:amount xmlns:epd="http://www.iai.kit.edu/EPD/2013" epd:module="D">-5.013431999999999E-6</epd:amount>
                <epd:referenceToUnitGroupDataSet xmlns:epd="http://www.iai.kit.edu/EPD/2013" refObjectId="54ccd2d9-a32a-4fc2-923d-f2c8c93e89d4" type="unit group data set" uri="../unitgroups/54ccd2d9-a32a-4fc2-923d-f2c8c93e89d4">
                    <common:shortDescription>kg Sb-Äqv.</common:shortDescription>
                </epd:referenceToUnitGroupDataSet>
            </common:other>
        </LCIAResult>
        <LCIAResult>
            <referenceToLCIAMethodDataSet type="LCIA method data set" refObjectId="804ebcdf-309d-4098-8ed8-fdaf2f389981" version="00.01.000">
                <common:shortDescription xml:lang="en">Abiotic depletion potential for fossil resources (ADPF)</common:shortDescription>
                <common:shortDescription xml:lang="de">Potenzial für den abiotischen Abbau fossiler Brennstoffe (ADPF)</common:shortDescription>
                <common:shortDescription xml:lang="es">Potencial de agotamiento de recursos abióticos para recursos fósiles (ADPF)</common:shortDescription>
            </referenceToLCIAMethodDataSet>
            <meanAmount>0.0</meanAmount>
            <common:other>
                <epd:amount xmlns:epd="http://www.iai.kit.edu/EPD/2013" epd:module="A1-A3">641.67</epd:amount>
                <epd:amount xmlns:epd="http://www.iai.kit.edu/EPD/2013" epd:module="C1">1.8771240000000002</epd:amount>
                <epd:amount xmlns:epd="http://www.iai.kit.edu/EPD/2013" epd:module="C2">0.7951920000000001</epd:amount>
                <epd:amount xmlns:epd="http://www.iai.kit.edu/EPD/2013" epd:module="C3">2.7349680000000003</epd:amount>
                <epd:amount xmlns:epd="http://www.iai.kit.edu/EPD/2013" epd:module="C4">2.230602</epd:amount>
                <epd:amount xmlns:epd="http://www.iai.kit.edu/EPD/2013" epd:module="D">-31.4541</epd:amount>
                <epd:referenceToUnitGroupDataSet xmlns:epd="http://www.iai.kit.edu/EPD/2013" refObjectId="93a60a57-a3c8-11da-a746-0800200c9a66" type="unit group data set" uri="../unitgroups/93a60a57-a3c8-11da-a746-0800200c9a66">
                    <common:shortDescription>MJ</common:shortDescription>
                </epd:referenceToUnitGroupDataSet>
            </common:other>
        </LCIAResult>
        <LCIAResult>
            <referenceToLCIAMethodDataSet type="LCIA method data set" refObjectId="b4274add-93b7-4905-a5e4-2e878c4e4216" version="00.01.000">
                <common:shortDescription xml:lang="en">Acidification potential of soil and water (AP)</common:shortDescription>
                <common:shortDescription xml:lang="de">Versauerungspotenzial von Boden und Wasser (AP)</common:shortDescription>
                <common:shortDescription xml:lang="es">Potencial de acidificación del suelo y de los recursos de agua (AP)</common:shortDescription>
            </referenceToLCIAMethodDataSet>
            <meanAmount>0.0</meanAmount>
            <common:other>
                <epd:amount xmlns:epd="http://www.iai.kit.edu/EPD/2013" epd:module="A1-A3">0.2944908</epd:amount>
                <epd:amount xmlns:epd="http://www.iai.kit.edu/EPD/2013" epd:module="C1">5.007852E-4</epd:amount>
                <epd:amount xmlns:epd="http://www.iai.kit.edu/EPD/2013" epd:module="C2">3.3906720000000004E-4</epd:amount>
                <epd:amount xmlns:epd="http://www.iai.kit.edu/EPD/2013" epd:module="C3">7.29642E-4</epd:amount>
                <epd:amount xmlns:epd="http://www.iai.kit.edu/EPD/2013" epd:module="C4">0.001021596</epd:amount>
                <epd:amount xmlns:epd="http://www.iai.kit.edu/EPD/2013" epd:module="D">-0.012645660000000001</epd:amount>
                <epd:referenceToUnitGroupDataSet xmlns:epd="http://www.iai.kit.edu/EPD/2013" refObjectId="bc50c624-a9bc-45b1-a9b0-e6b10d00476f" type="unit group data set" uri="../unitgroups/bc50c624-a9bc-45b1-a9b0-e6b10d00476f">
                    <common:shortDescription>kg SO2-Äqv.</common:shortDescription>
                </epd:referenceToUnitGroupDataSet>
            </common:other>
        </LCIAResult>
        <LCIAResult>
            <referenceToLCIAMethodDataSet type="LCIA method data set" refObjectId="f58827d0-b407-4ec6-be75-8b69efb98a0f" version="00.01.000">
                <common:shortDescription xml:lang="en">Eutrophication potential (EP)</common:shortDescription>
                <common:shortDescription xml:lang="de">Eutrophierungspotenzial (EP)</common:shortDescription>
                <common:shortDescription xml:lang="es">Potencial de eutrofización (EP)</common:shortDescription>
            </referenceToLCIAMethodDataSet>
            <meanAmount>0.0</meanAmount>
            <common:other>
                <epd:amount xmlns:epd="http://www.iai.kit.edu/EPD/2013" epd:module="A1-A3">0.02555268</epd:amount>
                <epd:amount xmlns:epd="http://www.iai.kit.edu/EPD/2013" epd:module="C1">4.692384E-5</epd:amount>
                <epd:amount xmlns:epd="http://www.iai.kit.edu/EPD/2013" epd:module="C2">8.71476E-5</epd:amount>
                <epd:amount xmlns:epd="http://www.iai.kit.edu/EPD/2013" epd:module="C3">6.83682E-5</epd:amount>
                <epd:amount xmlns:epd="http://www.iai.kit.edu/EPD/2013" epd:module="C4">1.4104500000000002E-4</epd:amount>
                <epd:amount xmlns:epd="http://www.iai.kit.edu/EPD/2013" epd:module="D">-0.001628736</epd:amount>
                <epd:referenceToUnitGroupDataSet xmlns:epd="http://www.iai.kit.edu/EPD/2013" refObjectId="67b5401d-873c-485f-bcf3-6ae83b918822" type="unit group data set" uri="../unitgroups/67b5401d-873c-485f-bcf3-6ae83b918822">
                    <common:shortDescription>kg Phosphat-Äqv.</common:shortDescription>
                </epd:referenceToUnitGroupDataSet>
            </common:other>
        </LCIAResult>
        <LCIAResult>
            <referenceToLCIAMethodDataSet type="LCIA method data set" refObjectId="77e416eb-a363-4258-a04e-171d843a6460" version="00.01.000">
                <common:shortDescription xml:lang="en">Global warming potential (GWP)</common:shortDescription>
                <common:shortDescription xml:lang="de">Globales Erwärmungspotenzial (GWP)</common:shortDescription>
                <common:shortDescription xml:lang="es">Potencial de calentamiento global (GWP)</common:shortDescription>
            </referenceToLCIAMethodDataSet>
            <meanAmount>0.0</meanAmount>
            <common:other>
                <epd:amount xmlns:epd="http://www.iai.kit.edu/EPD/2013" epd:module="A1-A3">47.5794</epd:amount>
                <epd:amount xmlns:epd="http://www.iai.kit.edu/EPD/2013" epd:module="C1">0.1763616</epd:amount>
                <epd:amount xmlns:epd="http://www.iai.kit.edu/EPD/2013" epd:module="C2">0.05780736</epd:amount>
                <epd:amount xmlns:epd="http://www.iai.kit.edu/EPD/2013" epd:module="C3">0.25695900000000005</epd:amount>
                <epd:amount xmlns:epd="http://www.iai.kit.edu/EPD/2013" epd:module="C4">0.172656</epd:amount>
                <epd:amount xmlns:epd="http://www.iai.kit.edu/EPD/2013" epd:module="D">-2.3170800000000003</epd:amount>
                <epd:referenceToUnitGroupDataSet xmlns:epd="http://www.iai.kit.edu/EPD/2013" refObjectId="1ebf3012-d0db-4de2-aefd-ef30cedb0be1" type="unit group data set" uri="../unitgroups/1ebf3012-d0db-4de2-aefd-ef30cedb0be1">
                    <common:shortDescription>kg CO2-Äqv.</common:shortDescription>
                </epd:referenceToUnitGroupDataSet>
            </common:other>
        </LCIAResult>
        <LCIAResult>
            <referenceToLCIAMethodDataSet type="LCIA method data set" refObjectId="06dcd26f-025f-401a-a7c1-5e457eb54637" version="00.01.000">
                <common:shortDescription xml:lang="en">Depletion potential of the stratospheric ozone layer (ODP)</common:shortDescription>
                <common:shortDescription xml:lang="de">Abbau Potential der stratosphärischen Ozonschicht (ODP)</common:shortDescription>
                <common:shortDescription xml:lang="es">Potencial de agotamiento de la capa de ozono estratosférico (ODP)</common:shortDescription>
            </referenceToLCIAMethodDataSet>
            <meanAmount>0.0</meanAmount>
            <common:other>
                <epd:amount xmlns:epd="http://www.iai.kit.edu/EPD/2013" epd:module="A1-A3">4.5606420000000006E-8</epd:amount>
                <epd:amount xmlns:epd="http://www.iai.kit.edu/EPD/2013" epd:module="C1">7.839780000000001E-13</epd:amount>
                <epd:amount xmlns:epd="http://www.iai.kit.edu/EPD/2013" epd:module="C2">1.596528E-15</epd:amount>
                <epd:amount xmlns:epd="http://www.iai.kit.edu/EPD/2013" epd:module="C3">1.1422560000000001E-12</epd:amount>
                <epd:amount xmlns:epd="http://www.iai.kit.edu/EPD/2013" epd:module="C4">3.9166259999999997E-14</epd:amount>
                <epd:amount xmlns:epd="http://www.iai.kit.edu/EPD/2013" epd:module="D">-1.34778E-12</epd:amount>
                <epd:referenceToUnitGroupDataSet xmlns:epd="http://www.iai.kit.edu/EPD/2013" refObjectId="88054749-b0a6-47ea-a82b-dc5b29326512" type="unit group data set" uri="../unitgroups/88054749-b0a6-47ea-a82b-dc5b29326512">
                    <common:shortDescription>kg CFC 11 eq.</common:shortDescription>
                </epd:referenceToUnitGroupDataSet>
            </common:other>
        </LCIAResult>
        <LCIAResult>
            <referenceToLCIAMethodDataSet type="LCIA method data set" refObjectId="1e84a202-dae6-42aa-9e9d-71ea48b8be00" version="00.01.000">
                <common:shortDescription xml:lang="en">Formation potential of tropospheric ozone (POCP)</common:shortDescription>
                <common:shortDescription xml:lang="de">Bildungspotential für troposphärisches Ozon (POCP)</common:shortDescription>
                <common:shortDescription xml:lang="es">Potencial de formación de ozono troposférico (POCP)</common:shortDescription>
            </referenceToLCIAMethodDataSet>
            <meanAmount>0.0</meanAmount>
            <common:other>
                <epd:amount xmlns:epd="http://www.iai.kit.edu/EPD/2013" epd:module="A1-A3">0.01760646</epd:amount>
                <epd:amount xmlns:epd="http://www.iai.kit.edu/EPD/2013" epd:module="C1">3.135042E-5</epd:amount>
                <epd:amount xmlns:epd="http://www.iai.kit.edu/EPD/2013" epd:module="C2">-1.51797E-4</epd:amount>
                <epd:amount xmlns:epd="http://www.iai.kit.edu/EPD/2013" epd:module="C3">4.567758E-5</epd:amount>
                <epd:amount xmlns:epd="http://www.iai.kit.edu/EPD/2013" epd:module="C4">7.94118E-5</epd:amount>
                <epd:amount xmlns:epd="http://www.iai.kit.edu/EPD/2013" epd:module="D">0.001773564</epd:amount>
                <epd:referenceToUnitGroupDataSet xmlns:epd="http://www.iai.kit.edu/EPD/2013" refObjectId="01c26c17-9a76-406e-8295-f17b55fd909e" type="unit group data set" uri="../unitgroups/01c26c17-9a76-406e-8295-f17b55fd909e">
                    <common:shortDescription>kg Ethen-Äqv.</common:shortDescription>
                </epd:referenceToUnitGroupDataSet>
            </common:other>
        </LCIAResult>
    </LCIAResults>
</processDataSet>
