<?xml version="1.0" encoding="utf-8"?>
<processDataSet xmlns:epd="http://www.iai.kit.edu/EPD/2013" xmlns:common="http://lca.jrc.it/ILCD/Common" xsi:schemaLocation="http://lca.jrc.it/ILCD/Process ../../schemas/EPD_DataSet.xsd" version="1.1" locations="../ILCDLocations.xml" xmlns:xsi="http://www.w3.org/2001/XMLSchema-instance" xmlns="http://lca.jrc.it/ILCD/Process">
<processInformation>
<dataSetInformation>
<common:UUID>b3cff98b-5067-4e82-a76f-b2ce058665d0</common:UUID>
<name>
<baseName xml:lang="en">TensoSky®-System with Fluon® ETFE-FILM</baseName>
<functionalUnitFlowProperties xml:lang="en" />
</name>
<classificationInformation>
<common:classification name="OEKOBAU.DAT">
<common:class level="0" classId="6">Kunststoffe</common:class>
<common:class level="1" classId="6.6">Folien und Vliese</common:class>
<common:class level="2" classId="6.6.07">Technische Textilien</common:class>
</common:classification>
<common:classification name="IBUCategories">
<common:class level="0">02 Building products</common:class>
<common:class level="1">Roof coverings</common:class>
<common:class level="2">ETFE construction element</common:class>
</common:classification>
</classificationInformation>
<common:generalComment xml:lang="en">The ETFE construction element with the trade brand name TensoSky® consists of AGC Inc.FLUON®ETFE-film, aluminium and further components with a minor mass proportion. It can be fixed on structural systems, e.g. made of steel, wood or reinforced concrete. The structural system is not included in this EPD. The construction element includes between 1 and 5 ETFE-film layers (ETFE = ethylene tetrafluoroethylene) dependent on building physical, statical or design requirements. The ETFE-film thickness varies between 80µm and 500 µm depending on structural requirements. The individual ETFE-films are welded together, to get a planar or curved single layer or multiple-layers system. This EPD is based on a reference 3-layers system with a film thickness of 250 µm (outer/inner layer) and 100 µm (middle layer). The values for 1-, 2-, 4- and 5-layers systems are derived from this reference project.</common:generalComment>
</dataSetInformation>
<quantitativeReference>
<referenceToReferenceFlow>0</referenceToReferenceFlow>
</quantitativeReference>
<time>
<common:referenceYear>2019</common:referenceYear>
<common:dataSetValidUntil>2024</common:dataSetValidUntil>
</time>
<geography>
<locationOfOperationSupplyOrProduction location="RER" />
</geography>
<technology>
<technologyDescriptionAndIncludedProcesses xml:lang="en">Taiyo Europe&apos;s ETFE construction element with the trade brand name TensoSky®, consists of ETFE-foils AGC FLUON® ETFE-Film, frames of aluminium and further materials for minor components. It can be fixed on a structural system (substructure), for example made of steel (beams, ropes etc.), wood or reinforced concrete. The structural system is not included in this EPD. The TensoSky®-System includes between one and five ETFE-Film layers (ETFE = ethylene tetrafluoroethylene) depending on the building physic, static or design requirements and specifications. The ETFE-Film thickness varies between 80µm and 500 µm depending on structural requirements. The individual foils of ETFE are welded together, to get a planar, single- or double-curved single layer or multiple-layers system. The layers are stabilized with a nominal pretension of about 1.0 kN/m (± 0.35 kN/m), achieved mechanically, by pulling the layer towards the aluminium frame, or pneumatically, by application of an overpressure in the air volume enclosed by the ETFE-layers. In case of a multiple-layers system with pneumatic pretension the nominal overpressure amounts between approximately 200 Pa (0.2 kN/m) and 1000 Pa (1.0 kN/m²). Under external loads, like wind loads, the overpressure changes. This means a low-pressure air inflation system. For use and application of the product, the respective national and regional provisions at the place of use apply, in Europe for example the Eurocode and the corresponding national appendixes. The TensoSky®-System is a transparent optionally translucent construction element, used as roof-cladding, skylight, indoor ceiling, facade-cladding, curtain wall, window or as protective canopy. It is suitable for new buildings and refurbishment projects. It can be used as permanent, stationary, moveable, retractable or temporary structure for Leisure Parcs and Indoor Pools, Biospheres and Greenhouses, Infrastructure Buildings and Carparks, Shopping Centers and Malls, Administration Buildings and Educational Buildings, Hotels and Hospitals, Public Spaces and Stadia, but also for pavillons and stands on trade fairs and exhibitions. 
Technical data: 
The following technical data indicates the default values for the declared ETFE-film product at the time of delivery. Unless otherwise stated the following material data refer to an ETFE-film with a thickness of 200 µm: 
Declared unit: 
The declaration refers to 1 m² of the TensoSky®-System (3.93 kg/m² mass per unit area for all components) including 3 layers of FLUON® ETFE-film (1.05 kg/m² mass per unit area).</technologyDescriptionAndIncludedProcesses>
<technologicalApplicability xml:lang="en">The TensoSky®-System is a transparent or translucent construction element, used e.g. as cladding roof, skylight, canopy, curtain wall or facade. It is suitable for new buildings and refurbishments. It can be used as a permanent, stationary, moveable, retractable or temporary structure, e.g. for leisure parcs, indoor pools, biospheres, greenhouses, infrastructure buildings, carparks, shopping malls, administration and educational buildings, hotels, hospitals, museums, public spaces and stadia, but also for pavillons and stands on trade fairs and exhibitions.</technologicalApplicability>
<referenceToTechnologyFlowDiagrammOrPicture uri="../sources/d124cd38-a5df-48e3-a2cc-9ee1dc08bf75.xml" type="source data set" refObjectId="d124cd38-a5df-48e3-a2cc-9ee1dc08bf75">
<common:shortDescription xml:lang="en">Constructional data ETFE</common:shortDescription>
</referenceToTechnologyFlowDiagrammOrPicture>
<referenceToTechnologyFlowDiagrammOrPicture uri="../sources/87620511-8f2a-42a3-b337-f2c48b1ff3a7.xml" type="source data set" refObjectId="87620511-8f2a-42a3-b337-f2c48b1ff3a7">
<common:shortDescription xml:lang="en">Declared unit</common:shortDescription>
</referenceToTechnologyFlowDiagrammOrPicture>
</technology>
</processInformation>
<modellingAndValidation>
<LCIMethodAndAllocation>
<typeOfDataSet>EPD</typeOfDataSet>
<referenceToLCAMethodDetails type="source data set" refObjectId="d44b24d7-41a1-4112-b8b4-c6a0b8248edd">
<common:shortDescription xml:lang="en">ETFE construction element.pdf</common:shortDescription>
</referenceToLCAMethodDetails>
<common:other>
<epd:subType xmlns="http://www.iai.kit.edu/EPD/2013">average dataset</epd:subType>
</common:other>
</LCIMethodAndAllocation>
<dataSourcesTreatmentAndRepresentativeness>
<referenceToDataSource type="source data set" refObjectId="be42dc5f-60dd-4f2a-87b2-ca1367c91256">
<common:shortDescription xml:lang="en">TensoSky®-System with Fluon® ETFE-FILM.pdf</common:shortDescription>
</referenceToDataSource>
<referenceToDataSource type="source data set" refObjectId="28d74cc0-db8b-4d7e-bc44-5f6d56ce0c4a">
<common:shortDescription xml:lang="en">GaBi Database (all versions)</common:shortDescription>
</referenceToDataSource>
<referenceToDataSource type="source data set" refObjectId="feda7597-12a1-4bd5-93ef-4d8120877b78">
<common:shortDescription xml:lang="en">GaBi database SP35 2018</common:shortDescription>
</referenceToDataSource>
<useAdviceForDataSet xml:lang="en">Scope: 
This EPD refers to individual construction elements manufactured from ethylenetetrafluoroethylene (ETFE), aluminium and other components. The construction element is used e.g. for building envelopes, cladding roofs, skylights, canopies, curtain walls or facades. It is supplied by Taiyo Europe GmbH, under the brand trade name TensoSky®, here used with Fluon®ETFE-film from AGC Inc, Japan. The TensoSky®-System is designed, fabricated and packaged for specific projects.This EPD declares the life cycle analysis (LCA) for a specific 3-layers system. 
System boundary: 
The EPD of the ETFE construction element, includes the production as well as installation, use phase and the End of Life of the product. The following life cycle phases are considered:ProductionA1-A3 – Raw material supply, production of pre-products (ETFE-film, aluminium frame, further parts) and manufacturing. Transports of raw materials (ETFE-film, aluminium…) and components/ pre-products are included in A2InstallationA4 – Transport to building siteA5 – Initial installation into building (including packaging waste processing, energy and material for the assembly of the building element and the electricity effort for first inflation)Use stageB1 – Use / application: Release of substances to indoor air, soil and waterB2 – Maintenance: Cleaning, yearly check and replacement of worn and damaged parts   B6 – Operational energy use: Maintaining the cushion pressure for a period of one yearB7 – Operational water useEnd-of-lifeC1 – Deconstruction/ demolition (including only minor effort for the deconstruction of the building element)C2 – Transport to waste processing resp. recycling material processing,C3 – Waste processing for recovery and recycling (including the incineration of ETFE and plastics and the recycling of aluminum and steel) C4 – Disposal (landfilling)</useAdviceForDataSet>
</dataSourcesTreatmentAndRepresentativeness>
<validation>
<review type="Accredited third party review">
<common:referenceToNameOfReviewerAndInstitution uri="../contacts/d111dbec-b024-4be5-86c5-752d6eb2cf95.xml" type="contact data set" refObjectId="d111dbec-b024-4be5-86c5-752d6eb2cf95">
<common:shortDescription xml:lang="en">Institut Bauen und Umwelt e. V.</common:shortDescription>
</common:referenceToNameOfReviewerAndInstitution>
</review>
</validation>
<complianceDeclarations>
<compliance>
<common:referenceToComplianceSystem uri="../sources/b00f9ec0-7874-11e3-981f-0800200c9a66.xml" type="source data set" refObjectId="b00f9ec0-7874-11e3-981f-0800200c9a66">
<common:shortDescription xml:lang="en">DIN EN 15804</common:shortDescription>
</common:referenceToComplianceSystem>
</compliance>
<compliance>
<common:referenceToComplianceSystem uri="../sources/4f2eb655-6e44-4874-a95a-e28f5442cd4d.xml" type="source data set" refObjectId="4f2eb655-6e44-4874-a95a-e28f5442cd4d">
<common:shortDescription xml:lang="en">ISO 14025</common:shortDescription>
</common:referenceToComplianceSystem>
</compliance>
</complianceDeclarations>
</modellingAndValidation>
<administrativeInformation>
<dataEntryBy>
<common:timeStamp>2019-08-05T15:02:54.838</common:timeStamp>
<common:referenceToDataSetFormat uri="../sources/a97a0155-0234-4b87-b4ce-a45da52f2a40.xml" type="source data set" refObjectId="a97a0155-0234-4b87-b4ce-a45da52f2a40">
<common:shortDescription xml:lang="en">ILCD Format 1.1</common:shortDescription>
</common:referenceToDataSetFormat>
<common:referenceToDataSetFormat uri="../sources/cba73800-7874-11e3-981f-0800200c9a66.xml" type="source data set" refObjectId="cba73800-7874-11e3-981f-0800200c9a66">
<common:shortDescription xml:lang="en">EPD Data Format Extensions</common:shortDescription>
</common:referenceToDataSetFormat>
<common:referenceToPersonOrEntityEnteringTheData uri="../contacts/623edf96-39d1-4e6f-9892-674c7228546b.xml" type="contact data set" refObjectId="623edf96-39d1-4e6f-9892-674c7228546b">
<common:shortDescription xml:lang="en">thinkstep AG</common:shortDescription>
</common:referenceToPersonOrEntityEnteringTheData>
</dataEntryBy>
<publicationAndOwnership>
<common:dataSetVersion>00.01.000</common:dataSetVersion>
<common:referenceToRegistrationAuthority uri="../contacts/d111dbec-b024-4be5-86c5-752d6eb2cf95.xml" type="contact data set" refObjectId="d111dbec-b024-4be5-86c5-752d6eb2cf95">
<common:shortDescription xml:lang="en">Institut Bauen und Umwelt e. V.</common:shortDescription>
</common:referenceToRegistrationAuthority>
<common:registrationNumber>11037</common:registrationNumber>
<common:referenceToOwnershipOfDataSet uri="../contacts/211efe4b-f094-46f0-bcdf-c76086d130c1.xml" type="contact data set" refObjectId="211efe4b-f094-46f0-bcdf-c76086d130c1">
<common:shortDescription xml:lang="en">Taiyo Europe GmbH</common:shortDescription>
</common:referenceToOwnershipOfDataSet>
<common:copyright>true</common:copyright>
</publicationAndOwnership>
</administrativeInformation>
<exchanges>
<exchange dataSetInternalID="0">
<referenceToFlowDataSet uri="../flows/fd06dc48-9622-7344-e76b-e02fdae613e0.xml" type="flow data set" refObjectId="fd06dc48-9622-7344-e76b-e02fdae613e0">
<common:shortDescription xml:lang="en">Taiyo ETFE construction element TensoSky / 1 m² ()</common:shortDescription>
</referenceToFlowDataSet>
<meanAmount>1</meanAmount>
<referencesToDataSource />
</exchange>
<exchange dataSetInternalID="1">
<referenceToFlowDataSet uri="../flows/20f32be5-0398-4288-9b6d-accddd195317.xml" type="flow data set" refObjectId="20f32be5-0398-4288-9b6d-accddd195317">
<common:shortDescription xml:lang="en">Renewable primary energy as energy carrier (PERE)</common:shortDescription>
</referenceToFlowDataSet>
<functionType>General reminder flow</functionType>
<exchangeDirection>Input</exchangeDirection>
<referencesToDataSource />
<common:other>
<epd:referenceToUnitGroupDataSet uri="../unitgroups/93a60a57-a3c8-11da-a746-0800200c9a66.xml" type="unit group data set" refObjectId="93a60a57-a3c8-11da-a746-0800200c9a66">
<common:shortDescription xml:lang="en">MJ</common:shortDescription>
</epd:referenceToUnitGroupDataSet>
<epd:amount epd:module="A1-A3">67.54</epd:amount>
<epd:amount epd:module="A4">0</epd:amount>
<epd:amount epd:module="A5">6.06172</epd:amount>
<epd:amount epd:module="B1">0</epd:amount>
<epd:amount epd:module="B2">0</epd:amount>
<epd:amount epd:module="B6">0.741</epd:amount>
<epd:amount epd:module="B7">0</epd:amount>
<epd:amount epd:module="C1">0</epd:amount>
<epd:amount epd:module="C2">0.03984</epd:amount>
<epd:amount epd:module="C3">0.1826</epd:amount>
<epd:amount epd:module="C4">0</epd:amount>
<epd:amount epd:module="D">-44.08</epd:amount>
</common:other>
</exchange>
<exchange dataSetInternalID="2">
<referenceToFlowDataSet uri="../flows/fb3ec0de-548d-4508-aea5-00b73bf6f702.xml" type="flow data set" refObjectId="fb3ec0de-548d-4508-aea5-00b73bf6f702">
<common:shortDescription xml:lang="en">Renewable primary energy resources as material utilization (PERM)</common:shortDescription>
</referenceToFlowDataSet>
<functionType>General reminder flow</functionType>
<exchangeDirection>Input</exchangeDirection>
<referencesToDataSource />
<common:other>
<epd:referenceToUnitGroupDataSet uri="../unitgroups/93a60a57-a3c8-11da-a746-0800200c9a66.xml" type="unit group data set" refObjectId="93a60a57-a3c8-11da-a746-0800200c9a66">
<common:shortDescription xml:lang="en">MJ</common:shortDescription>
</epd:referenceToUnitGroupDataSet>
<epd:amount epd:module="A1-A3">6.02</epd:amount>
<epd:amount epd:module="A4">0</epd:amount>
<epd:amount epd:module="A5">-6.02</epd:amount>
<epd:amount epd:module="B1">0</epd:amount>
<epd:amount epd:module="B2">0</epd:amount>
<epd:amount epd:module="B6">0</epd:amount>
<epd:amount epd:module="B7">0</epd:amount>
<epd:amount epd:module="C1">0</epd:amount>
<epd:amount epd:module="C2">0</epd:amount>
<epd:amount epd:module="C3">0</epd:amount>
<epd:amount epd:module="C4">0</epd:amount>
<epd:amount epd:module="D">0</epd:amount>
</common:other>
</exchange>
<exchange dataSetInternalID="3">
<referenceToFlowDataSet uri="../flows/53f97275-fa8a-4cdd-9024-65936002acd0.xml" type="flow data set" refObjectId="53f97275-fa8a-4cdd-9024-65936002acd0">
<common:shortDescription xml:lang="en">Total use of renewable primary energy resources (PERT)</common:shortDescription>
</referenceToFlowDataSet>
<functionType>General reminder flow</functionType>
<exchangeDirection>Input</exchangeDirection>
<referencesToDataSource />
<common:other>
<epd:referenceToUnitGroupDataSet uri="../unitgroups/93a60a57-a3c8-11da-a746-0800200c9a66.xml" type="unit group data set" refObjectId="93a60a57-a3c8-11da-a746-0800200c9a66">
<common:shortDescription xml:lang="en">MJ</common:shortDescription>
</epd:referenceToUnitGroupDataSet>
<epd:amount epd:module="A1-A3">73.56</epd:amount>
<epd:amount epd:module="A4">0</epd:amount>
<epd:amount epd:module="A5">0.04172</epd:amount>
<epd:amount epd:module="B1">0</epd:amount>
<epd:amount epd:module="B2">0</epd:amount>
<epd:amount epd:module="B6">0.741</epd:amount>
<epd:amount epd:module="B7">0</epd:amount>
<epd:amount epd:module="C1">0</epd:amount>
<epd:amount epd:module="C2">0.03984</epd:amount>
<epd:amount epd:module="C3">0.1826</epd:amount>
<epd:amount epd:module="C4">0</epd:amount>
<epd:amount epd:module="D">-44.08</epd:amount>
</common:other>
</exchange>
<exchange dataSetInternalID="4">
<referenceToFlowDataSet uri="../flows/ac857178-2b45-46ec-892a-a9a4332f0372.xml" type="flow data set" refObjectId="ac857178-2b45-46ec-892a-a9a4332f0372">
<common:shortDescription xml:lang="en">Non renewable primary energy as energy carrier (PENRE)</common:shortDescription>
</referenceToFlowDataSet>
<functionType>General reminder flow</functionType>
<exchangeDirection>Input</exchangeDirection>
<referencesToDataSource />
<common:other>
<epd:referenceToUnitGroupDataSet uri="../unitgroups/93a60a57-a3c8-11da-a746-0800200c9a66.xml" type="unit group data set" refObjectId="93a60a57-a3c8-11da-a746-0800200c9a66">
<common:shortDescription xml:lang="en">MJ</common:shortDescription>
</epd:referenceToUnitGroupDataSet>
<epd:amount epd:module="A1-A3">486.368</epd:amount>
<epd:amount epd:module="A4">0</epd:amount>
<epd:amount epd:module="A5">0.3814</epd:amount>
<epd:amount epd:module="B1">0</epd:amount>
<epd:amount epd:module="B2">0</epd:amount>
<epd:amount epd:module="B6">1.97</epd:amount>
<epd:amount epd:module="B7">0</epd:amount>
<epd:amount epd:module="C1">0</epd:amount>
<epd:amount epd:module="C2">0.7223</epd:amount>
<epd:amount epd:module="C3">27.1949</epd:amount>
<epd:amount epd:module="C4">0</epd:amount>
<epd:amount epd:module="D">-119.2</epd:amount>
</common:other>
</exchange>
<exchange dataSetInternalID="5">
<referenceToFlowDataSet uri="../flows/1421caa0-679d-4bf4-b282-0eb850ccae27.xml" type="flow data set" refObjectId="1421caa0-679d-4bf4-b282-0eb850ccae27">
<common:shortDescription xml:lang="en">Non renewable primary energy as material utilization (PENRM)</common:shortDescription>
</referenceToFlowDataSet>
<functionType>General reminder flow</functionType>
<exchangeDirection>Input</exchangeDirection>
<referencesToDataSource />
<common:other>
<epd:referenceToUnitGroupDataSet uri="../unitgroups/93a60a57-a3c8-11da-a746-0800200c9a66.xml" type="unit group data set" refObjectId="93a60a57-a3c8-11da-a746-0800200c9a66">
<common:shortDescription xml:lang="en">MJ</common:shortDescription>
</epd:referenceToUnitGroupDataSet>
<epd:amount epd:module="A1-A3">26.432</epd:amount>
<epd:amount epd:module="A4">0</epd:amount>
<epd:amount epd:module="A5">-0.16</epd:amount>
<epd:amount epd:module="B1">0</epd:amount>
<epd:amount epd:module="B2">0</epd:amount>
<epd:amount epd:module="B6">0</epd:amount>
<epd:amount epd:module="B7">0</epd:amount>
<epd:amount epd:module="C1">0</epd:amount>
<epd:amount epd:module="C2">0</epd:amount>
<epd:amount epd:module="C3">-26.272</epd:amount>
<epd:amount epd:module="C4">0</epd:amount>
<epd:amount epd:module="D">0</epd:amount>
</common:other>
</exchange>
<exchange dataSetInternalID="6">
<referenceToFlowDataSet uri="../flows/06159210-646b-4c8d-8583-da9b3b95a6c1.xml" type="flow data set" refObjectId="06159210-646b-4c8d-8583-da9b3b95a6c1">
<common:shortDescription xml:lang="en">Total use of non renewable primary energy resources (PENRT)</common:shortDescription>
</referenceToFlowDataSet>
<functionType>General reminder flow</functionType>
<exchangeDirection>Input</exchangeDirection>
<referencesToDataSource />
<common:other>
<epd:referenceToUnitGroupDataSet uri="../unitgroups/93a60a57-a3c8-11da-a746-0800200c9a66.xml" type="unit group data set" refObjectId="93a60a57-a3c8-11da-a746-0800200c9a66">
<common:shortDescription xml:lang="en">MJ</common:shortDescription>
</epd:referenceToUnitGroupDataSet>
<epd:amount epd:module="A1-A3">512.8</epd:amount>
<epd:amount epd:module="A4">0</epd:amount>
<epd:amount epd:module="A5">0.2214</epd:amount>
<epd:amount epd:module="B1">0</epd:amount>
<epd:amount epd:module="B2">0</epd:amount>
<epd:amount epd:module="B6">1.97</epd:amount>
<epd:amount epd:module="B7">0</epd:amount>
<epd:amount epd:module="C1">0</epd:amount>
<epd:amount epd:module="C2">0.7223</epd:amount>
<epd:amount epd:module="C3">0.9229</epd:amount>
<epd:amount epd:module="C4">0</epd:amount>
<epd:amount epd:module="D">-119.2</epd:amount>
</common:other>
</exchange>
<exchange dataSetInternalID="7">
<referenceToFlowDataSet uri="../flows/c6a1f35f-2d09-4f54-8dfb-97e502e1ce92.xml" type="flow data set" refObjectId="c6a1f35f-2d09-4f54-8dfb-97e502e1ce92">
<common:shortDescription xml:lang="en">Use of secondary material (SM)</common:shortDescription>
</referenceToFlowDataSet>
<functionType>General reminder flow</functionType>
<exchangeDirection>Input</exchangeDirection>
<referencesToDataSource />
<common:other>
<epd:referenceToUnitGroupDataSet uri="../unitgroups/ad38d542-3fe9-439d-9b95-2f5f7752acaf.xml" type="unit group data set" refObjectId="ad38d542-3fe9-439d-9b95-2f5f7752acaf">
<common:shortDescription xml:lang="en">kg</common:shortDescription>
</epd:referenceToUnitGroupDataSet>
<epd:amount epd:module="A1-A3">0.85</epd:amount>
<epd:amount epd:module="A4">0</epd:amount>
<epd:amount epd:module="A5">0</epd:amount>
<epd:amount epd:module="B1">0</epd:amount>
<epd:amount epd:module="B2">0</epd:amount>
<epd:amount epd:module="B6">0</epd:amount>
<epd:amount epd:module="B7">0</epd:amount>
<epd:amount epd:module="C1">0</epd:amount>
<epd:amount epd:module="C2">0</epd:amount>
<epd:amount epd:module="C3">0</epd:amount>
<epd:amount epd:module="C4">0</epd:amount>
<epd:amount epd:module="D">0</epd:amount>
</common:other>
</exchange>
<exchange dataSetInternalID="8">
<referenceToFlowDataSet uri="../flows/64333088-a55f-4aa2-9a31-c10b07816787.xml" type="flow data set" refObjectId="64333088-a55f-4aa2-9a31-c10b07816787">
<common:shortDescription xml:lang="en">Use of renewable secondary fuels (RSF)</common:shortDescription>
</referenceToFlowDataSet>
<functionType>General reminder flow</functionType>
<exchangeDirection>Input</exchangeDirection>
<referencesToDataSource />
<common:other>
<epd:referenceToUnitGroupDataSet uri="../unitgroups/93a60a57-a3c8-11da-a746-0800200c9a66.xml" type="unit group data set" refObjectId="93a60a57-a3c8-11da-a746-0800200c9a66">
<common:shortDescription xml:lang="en">MJ</common:shortDescription>
</epd:referenceToUnitGroupDataSet>
<epd:amount epd:module="A1-A3">0</epd:amount>
<epd:amount epd:module="A4">0</epd:amount>
<epd:amount epd:module="A5">0</epd:amount>
<epd:amount epd:module="B1">0</epd:amount>
<epd:amount epd:module="B2">0</epd:amount>
<epd:amount epd:module="B6">0</epd:amount>
<epd:amount epd:module="B7">0</epd:amount>
<epd:amount epd:module="C1">0</epd:amount>
<epd:amount epd:module="C2">0</epd:amount>
<epd:amount epd:module="C3">0</epd:amount>
<epd:amount epd:module="C4">0</epd:amount>
<epd:amount epd:module="D">0</epd:amount>
</common:other>
</exchange>
<exchange dataSetInternalID="9">
<referenceToFlowDataSet uri="../flows/89def144-d39a-4287-b86f-efde453ddcb2.xml" type="flow data set" refObjectId="89def144-d39a-4287-b86f-efde453ddcb2">
<common:shortDescription xml:lang="en">Use of non renewable secondary fuels (NRSF)</common:shortDescription>
</referenceToFlowDataSet>
<functionType>General reminder flow</functionType>
<exchangeDirection>Input</exchangeDirection>
<referencesToDataSource />
<common:other>
<epd:referenceToUnitGroupDataSet uri="../unitgroups/93a60a57-a3c8-11da-a746-0800200c9a66.xml" type="unit group data set" refObjectId="93a60a57-a3c8-11da-a746-0800200c9a66">
<common:shortDescription xml:lang="en">MJ</common:shortDescription>
</epd:referenceToUnitGroupDataSet>
<epd:amount epd:module="A1-A3">0</epd:amount>
<epd:amount epd:module="A4">0</epd:amount>
<epd:amount epd:module="A5">0</epd:amount>
<epd:amount epd:module="B1">0</epd:amount>
<epd:amount epd:module="B2">0</epd:amount>
<epd:amount epd:module="B6">0</epd:amount>
<epd:amount epd:module="B7">0</epd:amount>
<epd:amount epd:module="C1">0</epd:amount>
<epd:amount epd:module="C2">0</epd:amount>
<epd:amount epd:module="C3">0</epd:amount>
<epd:amount epd:module="C4">0</epd:amount>
<epd:amount epd:module="D">0</epd:amount>
</common:other>
</exchange>
<exchange dataSetInternalID="10">
<referenceToFlowDataSet uri="../flows/3cf952c8-f3a4-461d-8c96-96456ca62246.xml" type="flow data set" refObjectId="3cf952c8-f3a4-461d-8c96-96456ca62246">
<common:shortDescription xml:lang="en">Use of net fresh water (FW)</common:shortDescription>
</referenceToFlowDataSet>
<functionType>General reminder flow</functionType>
<exchangeDirection>Input</exchangeDirection>
<referencesToDataSource />
<common:other>
<epd:referenceToUnitGroupDataSet uri="../unitgroups/cd950537-0a98-4044-9ba7-9f9a68d0a504.xml" type="unit group data set" refObjectId="cd950537-0a98-4044-9ba7-9f9a68d0a504">
<common:shortDescription xml:lang="en">m^3</common:shortDescription>
</epd:referenceToUnitGroupDataSet>
<epd:amount epd:module="A1-A3">0.2394</epd:amount>
<epd:amount epd:module="A4">0</epd:amount>
<epd:amount epd:module="A5">0.002217</epd:amount>
<epd:amount epd:module="B1">0</epd:amount>
<epd:amount epd:module="B2">0</epd:amount>
<epd:amount epd:module="B6">0.00101</epd:amount>
<epd:amount epd:module="B7">0</epd:amount>
<epd:amount epd:module="C1">0</epd:amount>
<epd:amount epd:module="C2">7.341E-05</epd:amount>
<epd:amount epd:module="C3">0.006179</epd:amount>
<epd:amount epd:module="C4">0</epd:amount>
<epd:amount epd:module="D">-0.1105</epd:amount>
</common:other>
</exchange>
<exchange dataSetInternalID="11">
<referenceToFlowDataSet uri="../flows/430f9e0f-59b2-46a0-8e0d-55e0e84948fc.xml" type="flow data set" refObjectId="430f9e0f-59b2-46a0-8e0d-55e0e84948fc">
<common:shortDescription xml:lang="en">Hazardous waste disposed (HWD)</common:shortDescription>
</referenceToFlowDataSet>
<functionType>General reminder flow</functionType>
<exchangeDirection>Output</exchangeDirection>
<referencesToDataSource />
<common:other>
<epd:referenceToUnitGroupDataSet uri="../unitgroups/ad38d542-3fe9-439d-9b95-2f5f7752acaf.xml" type="unit group data set" refObjectId="ad38d542-3fe9-439d-9b95-2f5f7752acaf">
<common:shortDescription xml:lang="en">kg</common:shortDescription>
</epd:referenceToUnitGroupDataSet>
<epd:amount epd:module="A1-A3">0.001871</epd:amount>
<epd:amount epd:module="A4">0</epd:amount>
<epd:amount epd:module="A5">1.842E-10</epd:amount>
<epd:amount epd:module="B1">0</epd:amount>
<epd:amount epd:module="B2">0</epd:amount>
<epd:amount epd:module="B6">9.25E-10</epd:amount>
<epd:amount epd:module="B7">0</epd:amount>
<epd:amount epd:module="C1">0</epd:amount>
<epd:amount epd:module="C2">4.176E-08</epd:amount>
<epd:amount epd:module="C3">4.506E-08</epd:amount>
<epd:amount epd:module="C4">0</epd:amount>
<epd:amount epd:module="D">0.002497</epd:amount>
</common:other>
</exchange>
<exchange dataSetInternalID="12">
<referenceToFlowDataSet uri="../flows/b29ef66b-e286-4afa-949f-62f1a7b4d7fa.xml" type="flow data set" refObjectId="b29ef66b-e286-4afa-949f-62f1a7b4d7fa">
<common:shortDescription xml:lang="en">Non hazardous waste disposed (NHWD)</common:shortDescription>
</referenceToFlowDataSet>
<functionType>General reminder flow</functionType>
<exchangeDirection>Output</exchangeDirection>
<referencesToDataSource />
<common:other>
<epd:referenceToUnitGroupDataSet uri="../unitgroups/ad38d542-3fe9-439d-9b95-2f5f7752acaf.xml" type="unit group data set" refObjectId="ad38d542-3fe9-439d-9b95-2f5f7752acaf">
<common:shortDescription xml:lang="en">kg</common:shortDescription>
</epd:referenceToUnitGroupDataSet>
<epd:amount epd:module="A1-A3">2.895</epd:amount>
<epd:amount epd:module="A4">0</epd:amount>
<epd:amount epd:module="A5">0.002198</epd:amount>
<epd:amount epd:module="B1">0</epd:amount>
<epd:amount epd:module="B2">0</epd:amount>
<epd:amount epd:module="B6">0.00139</epd:amount>
<epd:amount epd:module="B7">0</epd:amount>
<epd:amount epd:module="C1">0</epd:amount>
<epd:amount epd:module="C2">6.051E-05</epd:amount>
<epd:amount epd:module="C3">0.3388</epd:amount>
<epd:amount epd:module="C4">0</epd:amount>
<epd:amount epd:module="D">-1.95</epd:amount>
</common:other>
</exchange>
<exchange dataSetInternalID="13">
<referenceToFlowDataSet uri="../flows/3449546e-52ad-4b39-b809-9fb77cea8ff6.xml" type="flow data set" refObjectId="3449546e-52ad-4b39-b809-9fb77cea8ff6">
<common:shortDescription xml:lang="en">Radioactive waste disposed (RWD)</common:shortDescription>
</referenceToFlowDataSet>
<functionType>General reminder flow</functionType>
<exchangeDirection>Output</exchangeDirection>
<referencesToDataSource />
<common:other>
<epd:referenceToUnitGroupDataSet uri="../unitgroups/ad38d542-3fe9-439d-9b95-2f5f7752acaf.xml" type="unit group data set" refObjectId="ad38d542-3fe9-439d-9b95-2f5f7752acaf">
<common:shortDescription xml:lang="en">kg</common:shortDescription>
</epd:referenceToUnitGroupDataSet>
<epd:amount epd:module="A1-A3">0.01358</epd:amount>
<epd:amount epd:module="A4">0</epd:amount>
<epd:amount epd:module="A5">9.422E-06</epd:amount>
<epd:amount epd:module="B1">0</epd:amount>
<epd:amount epd:module="B2">0</epd:amount>
<epd:amount epd:module="B6">0.000327</epd:amount>
<epd:amount epd:module="B7">0</epd:amount>
<epd:amount epd:module="C1">0</epd:amount>
<epd:amount epd:module="C2">9.885E-07</epd:amount>
<epd:amount epd:module="C3">7.124E-05</epd:amount>
<epd:amount epd:module="C4">0</epd:amount>
<epd:amount epd:module="D">-0.007503</epd:amount>
</common:other>
</exchange>
<exchange dataSetInternalID="14">
<referenceToFlowDataSet uri="../flows/a2b32f97-3fc7-4af2-b209-525bc6426f33.xml" type="flow data set" refObjectId="a2b32f97-3fc7-4af2-b209-525bc6426f33">
<common:shortDescription xml:lang="en">Components for re-use (CRU)</common:shortDescription>
</referenceToFlowDataSet>
<functionType>General reminder flow</functionType>
<exchangeDirection>Output</exchangeDirection>
<referencesToDataSource />
<common:other>
<epd:referenceToUnitGroupDataSet uri="../unitgroups/ad38d542-3fe9-439d-9b95-2f5f7752acaf.xml" type="unit group data set" refObjectId="ad38d542-3fe9-439d-9b95-2f5f7752acaf">
<common:shortDescription xml:lang="en">kg</common:shortDescription>
</epd:referenceToUnitGroupDataSet>
<epd:amount epd:module="A1-A3">0</epd:amount>
<epd:amount epd:module="A4">0</epd:amount>
<epd:amount epd:module="A5">0</epd:amount>
<epd:amount epd:module="B1">0</epd:amount>
<epd:amount epd:module="B2">0</epd:amount>
<epd:amount epd:module="B6">0</epd:amount>
<epd:amount epd:module="B7">0</epd:amount>
<epd:amount epd:module="C1">0</epd:amount>
<epd:amount epd:module="C2">0</epd:amount>
<epd:amount epd:module="C3">0</epd:amount>
<epd:amount epd:module="C4">0</epd:amount>
<epd:amount epd:module="D">0</epd:amount>
</common:other>
</exchange>
<exchange dataSetInternalID="15">
<referenceToFlowDataSet uri="../flows/d7fe48a5-4103-49c8-9aae-b0b5dfdbd6ae.xml" type="flow data set" refObjectId="d7fe48a5-4103-49c8-9aae-b0b5dfdbd6ae">
<common:shortDescription xml:lang="en">Materials for recycling (MFR)</common:shortDescription>
</referenceToFlowDataSet>
<functionType>General reminder flow</functionType>
<exchangeDirection>Output</exchangeDirection>
<referencesToDataSource />
<common:other>
<epd:referenceToUnitGroupDataSet uri="../unitgroups/ad38d542-3fe9-439d-9b95-2f5f7752acaf.xml" type="unit group data set" refObjectId="ad38d542-3fe9-439d-9b95-2f5f7752acaf">
<common:shortDescription xml:lang="en">kg</common:shortDescription>
</epd:referenceToUnitGroupDataSet>
<epd:amount epd:module="A1-A3">0</epd:amount>
<epd:amount epd:module="A4">0</epd:amount>
<epd:amount epd:module="A5">0</epd:amount>
<epd:amount epd:module="B1">0</epd:amount>
<epd:amount epd:module="B2">0</epd:amount>
<epd:amount epd:module="B6">0</epd:amount>
<epd:amount epd:module="B7">0</epd:amount>
<epd:amount epd:module="C1">0</epd:amount>
<epd:amount epd:module="C2">0</epd:amount>
<epd:amount epd:module="C3">2.346</epd:amount>
<epd:amount epd:module="C4">0</epd:amount>
<epd:amount epd:module="D">0</epd:amount>
</common:other>
</exchange>
<exchange dataSetInternalID="16">
<referenceToFlowDataSet uri="../flows/59a9181c-3aaf-46ee-8b13-2b3723b6e447.xml" type="flow data set" refObjectId="59a9181c-3aaf-46ee-8b13-2b3723b6e447">
<common:shortDescription xml:lang="en">Materials for energy recovery (MER)</common:shortDescription>
</referenceToFlowDataSet>
<functionType>General reminder flow</functionType>
<exchangeDirection>Output</exchangeDirection>
<referencesToDataSource />
<common:other>
<epd:referenceToUnitGroupDataSet uri="../unitgroups/ad38d542-3fe9-439d-9b95-2f5f7752acaf.xml" type="unit group data set" refObjectId="ad38d542-3fe9-439d-9b95-2f5f7752acaf">
<common:shortDescription xml:lang="en">kg</common:shortDescription>
</epd:referenceToUnitGroupDataSet>
<epd:amount epd:module="A1-A3">0</epd:amount>
<epd:amount epd:module="A4">0</epd:amount>
<epd:amount epd:module="A5">0</epd:amount>
<epd:amount epd:module="B1">0</epd:amount>
<epd:amount epd:module="B2">0</epd:amount>
<epd:amount epd:module="B6">0</epd:amount>
<epd:amount epd:module="B7">0</epd:amount>
<epd:amount epd:module="C1">0</epd:amount>
<epd:amount epd:module="C2">0</epd:amount>
<epd:amount epd:module="C3">0</epd:amount>
<epd:amount epd:module="C4">0</epd:amount>
<epd:amount epd:module="D">0</epd:amount>
</common:other>
</exchange>
<exchange dataSetInternalID="17">
<referenceToFlowDataSet uri="../flows/4da0c987-2b76-40d6-9e9e-82a017aaaf29.xml" type="flow data set" refObjectId="4da0c987-2b76-40d6-9e9e-82a017aaaf29">
<common:shortDescription xml:lang="en">Exported electrical energy (EEE)</common:shortDescription>
</referenceToFlowDataSet>
<functionType>General reminder flow</functionType>
<exchangeDirection>Output</exchangeDirection>
<referencesToDataSource />
<common:other>
<epd:referenceToUnitGroupDataSet uri="../unitgroups/93a60a57-a3c8-11da-a746-0800200c9a66.xml" type="unit group data set" refObjectId="93a60a57-a3c8-11da-a746-0800200c9a66">
<common:shortDescription xml:lang="en">MJ</common:shortDescription>
</epd:referenceToUnitGroupDataSet>
<epd:amount epd:module="A1-A3">0</epd:amount>
<epd:amount epd:module="A4">0</epd:amount>
<epd:amount epd:module="A5">0.02282</epd:amount>
<epd:amount epd:module="B1">0</epd:amount>
<epd:amount epd:module="B2">0</epd:amount>
<epd:amount epd:module="B6">0</epd:amount>
<epd:amount epd:module="B7">0</epd:amount>
<epd:amount epd:module="C1">0</epd:amount>
<epd:amount epd:module="C2">0</epd:amount>
<epd:amount epd:module="C3">2.132</epd:amount>
<epd:amount epd:module="C4">0</epd:amount>
<epd:amount epd:module="D">0</epd:amount>
</common:other>
</exchange>
<exchange dataSetInternalID="18">
<referenceToFlowDataSet uri="../flows/98daf38a-7a79-46d3-9a37-2b7bd0955810.xml" type="flow data set" refObjectId="98daf38a-7a79-46d3-9a37-2b7bd0955810">
<common:shortDescription xml:lang="en">Exported thermal energy (EET)</common:shortDescription>
</referenceToFlowDataSet>
<functionType>General reminder flow</functionType>
<exchangeDirection>Output</exchangeDirection>
<referencesToDataSource />
<common:other>
<epd:referenceToUnitGroupDataSet uri="../unitgroups/93a60a57-a3c8-11da-a746-0800200c9a66.xml" type="unit group data set" refObjectId="93a60a57-a3c8-11da-a746-0800200c9a66">
<common:shortDescription xml:lang="en">MJ</common:shortDescription>
</epd:referenceToUnitGroupDataSet>
<epd:amount epd:module="A1-A3">0</epd:amount>
<epd:amount epd:module="A4">0</epd:amount>
<epd:amount epd:module="A5">0.05257</epd:amount>
<epd:amount epd:module="B1">0</epd:amount>
<epd:amount epd:module="B2">0</epd:amount>
<epd:amount epd:module="B6">0</epd:amount>
<epd:amount epd:module="B7">0</epd:amount>
<epd:amount epd:module="C1">0</epd:amount>
<epd:amount epd:module="C2">0</epd:amount>
<epd:amount epd:module="C3">3.83</epd:amount>
<epd:amount epd:module="C4">0</epd:amount>
<epd:amount epd:module="D">0</epd:amount>
</common:other>
</exchange>
</exchanges>
<LCIAResults>
<LCIAResult>
<referenceToLCIAMethodDataSet uri="../flows/77e416eb-a363-4258-a04e-171d843a6460.xml" type="LCIA method data set" refObjectId="77e416eb-a363-4258-a04e-171d843a6460">
<common:shortDescription xml:lang="en">Global warming potential (GWP)</common:shortDescription>
</referenceToLCIAMethodDataSet>
<common:other>
<epd:referenceToUnitGroupDataSet uri="../unitgroups/1ebf3012-d0db-4de2-aefd-ef30cedb0be1.xml" type="unit group data set" refObjectId="1ebf3012-d0db-4de2-aefd-ef30cedb0be1">
<common:shortDescription xml:lang="en">kg CO_(2)-Äq.</common:shortDescription>
</epd:referenceToUnitGroupDataSet>
<epd:amount epd:module="A1-A3">53.19</epd:amount>
<epd:amount epd:module="A4">0</epd:amount>
<epd:amount epd:module="A5">0.9161</epd:amount>
<epd:amount epd:module="B1">0</epd:amount>
<epd:amount epd:module="B2">0</epd:amount>
<epd:amount epd:module="B6">0.108</epd:amount>
<epd:amount epd:module="B7">0</epd:amount>
<epd:amount epd:module="C1">0</epd:amount>
<epd:amount epd:module="C2">0.05307</epd:amount>
<epd:amount epd:module="C3">2.253</epd:amount>
<epd:amount epd:module="C4">0</epd:amount>
<epd:amount epd:module="D">-9.365</epd:amount>
</common:other>
</LCIAResult>
<LCIAResult>
<referenceToLCIAMethodDataSet uri="../flows/06dcd26f-025f-401a-a7c1-5e457eb54637.xml" type="LCIA method data set" refObjectId="06dcd26f-025f-401a-a7c1-5e457eb54637">
<common:shortDescription xml:lang="en">Depletion potential of the stratospheric ozone layer (ODP)</common:shortDescription>
</referenceToLCIAMethodDataSet>
<common:other>
<epd:referenceToUnitGroupDataSet uri="../unitgroups/88054749-b0a6-47ea-a82b-dc5b29326512.xml" type="unit group data set" refObjectId="88054749-b0a6-47ea-a82b-dc5b29326512">
<common:shortDescription xml:lang="en">kg CFC11-Äq.</common:shortDescription>
</epd:referenceToUnitGroupDataSet>
<epd:amount epd:module="A1-A3">0.000267</epd:amount>
<epd:amount epd:module="A4">0</epd:amount>
<epd:amount epd:module="A5">1.116E-14</epd:amount>
<epd:amount epd:module="B1">0</epd:amount>
<epd:amount epd:module="B2">0</epd:amount>
<epd:amount epd:module="B6">4.8E-13</epd:amount>
<epd:amount epd:module="B7">0</epd:amount>
<epd:amount epd:module="C1">0</epd:amount>
<epd:amount epd:module="C2">1.445E-15</epd:amount>
<epd:amount epd:module="C3">9.986E-14</epd:amount>
<epd:amount epd:module="C4">0</epd:amount>
<epd:amount epd:module="D">4.133E-11</epd:amount>
</common:other>
</LCIAResult>
<LCIAResult>
<referenceToLCIAMethodDataSet uri="../flows/b4274add-93b7-4905-a5e4-2e878c4e4216.xml" type="LCIA method data set" refObjectId="b4274add-93b7-4905-a5e4-2e878c4e4216">
<common:shortDescription xml:lang="en">Acidification potential of land and water (AP)</common:shortDescription>
</referenceToLCIAMethodDataSet>
<common:other>
<epd:referenceToUnitGroupDataSet uri="../unitgroups/bc50c624-a9bc-45b1-a9b0-e6b10d00476f.xml" type="unit group data set" refObjectId="bc50c624-a9bc-45b1-a9b0-e6b10d00476f">
<common:shortDescription xml:lang="en">kg SO_(2)-Äq.</common:shortDescription>
</epd:referenceToUnitGroupDataSet>
<epd:amount epd:module="A1-A3">0.1083</epd:amount>
<epd:amount epd:module="A4">0</epd:amount>
<epd:amount epd:module="A5">0.0001109</epd:amount>
<epd:amount epd:module="B1">0</epd:amount>
<epd:amount epd:module="B2">0</epd:amount>
<epd:amount epd:module="B6">0.000306</epd:amount>
<epd:amount epd:module="B7">0</epd:amount>
<epd:amount epd:module="C1">0</epd:amount>
<epd:amount epd:module="C2">0.0001233</epd:amount>
<epd:amount epd:module="C3">0.02113</epd:amount>
<epd:amount epd:module="C4">0</epd:amount>
<epd:amount epd:module="D">-0.03991</epd:amount>
</common:other>
</LCIAResult>
<LCIAResult>
<referenceToLCIAMethodDataSet uri="../flows/f58827d0-b407-4ec6-be75-8b69efb98a0f.xml" type="LCIA method data set" refObjectId="f58827d0-b407-4ec6-be75-8b69efb98a0f">
<common:shortDescription xml:lang="en">Eutrophication potential (EP)</common:shortDescription>
</referenceToLCIAMethodDataSet>
<common:other>
<epd:referenceToUnitGroupDataSet uri="../unitgroups/67b5401d-873c-485f-bcf3-6ae83b918822.xml" type="unit group data set" refObjectId="67b5401d-873c-485f-bcf3-6ae83b918822">
<common:shortDescription xml:lang="en">kg PO_(4)^(3)-Äq.</common:shortDescription>
</epd:referenceToUnitGroupDataSet>
<epd:amount epd:module="A1-A3">0.008073</epd:amount>
<epd:amount epd:module="A4">0</epd:amount>
<epd:amount epd:module="A5">2.435E-05</epd:amount>
<epd:amount epd:module="B1">0</epd:amount>
<epd:amount epd:module="B2">0</epd:amount>
<epd:amount epd:module="B6">2.87E-05</epd:amount>
<epd:amount epd:module="B7">0</epd:amount>
<epd:amount epd:module="C1">0</epd:amount>
<epd:amount epd:module="C2">3.127E-05</epd:amount>
<epd:amount epd:module="C3">6.795E-05</epd:amount>
<epd:amount epd:module="C4">0</epd:amount>
<epd:amount epd:module="D">-0.002495</epd:amount>
</common:other>
</LCIAResult>
<LCIAResult>
<referenceToLCIAMethodDataSet uri="../flows/1e84a202-dae6-42aa-9e9d-71ea48b8be00.xml" type="LCIA method data set" refObjectId="1e84a202-dae6-42aa-9e9d-71ea48b8be00">
<common:shortDescription xml:lang="en">Formation potential of tropospheric ozone photochemical oxidants (POCP)</common:shortDescription>
</referenceToLCIAMethodDataSet>
<common:other>
<epd:referenceToUnitGroupDataSet uri="../unitgroups/01c26c17-9a76-406e-8295-f17b55fd909e.xml" type="unit group data set" refObjectId="01c26c17-9a76-406e-8295-f17b55fd909e">
<common:shortDescription xml:lang="en">kg Ethen-Äq.</common:shortDescription>
</epd:referenceToUnitGroupDataSet>
<epd:amount epd:module="A1-A3">0.009361</epd:amount>
<epd:amount epd:module="A4">0</epd:amount>
<epd:amount epd:module="A5">7.369E-06</epd:amount>
<epd:amount epd:module="B1">0</epd:amount>
<epd:amount epd:module="B2">0</epd:amount>
<epd:amount epd:module="B6">1.92E-05</epd:amount>
<epd:amount epd:module="B7">0</epd:amount>
<epd:amount epd:module="C1">0</epd:amount>
<epd:amount epd:module="C2">-4.167E-05</epd:amount>
<epd:amount epd:module="C3">3.019E-05</epd:amount>
<epd:amount epd:module="C4">0</epd:amount>
<epd:amount epd:module="D">-0.002434</epd:amount>
</common:other>
</LCIAResult>
<LCIAResult>
<referenceToLCIAMethodDataSet uri="../flows/f7c73bb9-ab1a-4249-9c6d-379a0de6f67e.xml" type="LCIA method data set" refObjectId="f7c73bb9-ab1a-4249-9c6d-379a0de6f67e">
<common:shortDescription xml:lang="en">Abiotic depletion potential for non fossil resources (ADPE)</common:shortDescription>
</referenceToLCIAMethodDataSet>
<common:other>
<epd:referenceToUnitGroupDataSet uri="../unitgroups/54ccd2d9-a32a-4fc2-923d-f2c8c93e89d4.xml" type="unit group data set" refObjectId="54ccd2d9-a32a-4fc2-923d-f2c8c93e89d4">
<common:shortDescription xml:lang="en">kg Sb-Äq.</common:shortDescription>
</epd:referenceToUnitGroupDataSet>
<epd:amount epd:module="A1-A3">0.0001452</epd:amount>
<epd:amount epd:module="A4">0</epd:amount>
<epd:amount epd:module="A5">1.295E-08</epd:amount>
<epd:amount epd:module="B1">0</epd:amount>
<epd:amount epd:module="B2">0</epd:amount>
<epd:amount epd:module="B6">5.73E-08</epd:amount>
<epd:amount epd:module="B7">0</epd:amount>
<epd:amount epd:module="C1">0</epd:amount>
<epd:amount epd:module="C2">4.342E-09</epd:amount>
<epd:amount epd:module="C3">2.644E-07</epd:amount>
<epd:amount epd:module="C4">0</epd:amount>
<epd:amount epd:module="D">-3.625E-06</epd:amount>
</common:other>
</LCIAResult>
<LCIAResult>
<referenceToLCIAMethodDataSet uri="../flows/804ebcdf-309d-4098-8ed8-fdaf2f389981.xml" type="LCIA method data set" refObjectId="804ebcdf-309d-4098-8ed8-fdaf2f389981">
<common:shortDescription xml:lang="en">Abiotic depletion potential for fossil resources (ADPF)</common:shortDescription>
</referenceToLCIAMethodDataSet>
<common:other>
<epd:referenceToUnitGroupDataSet uri="../unitgroups/93a60a57-a3c8-11da-a746-0800200c9a66.xml" type="unit group data set" refObjectId="93a60a57-a3c8-11da-a746-0800200c9a66">
<common:shortDescription xml:lang="en">MJ</common:shortDescription>
</epd:referenceToUnitGroupDataSet>
<epd:amount epd:module="A1-A3">487.6</epd:amount>
<epd:amount epd:module="A4">0</epd:amount>
<epd:amount epd:module="A5">0.1976</epd:amount>
<epd:amount epd:module="B1">0</epd:amount>
<epd:amount epd:module="B2">0</epd:amount>
<epd:amount epd:module="B6">1.15</epd:amount>
<epd:amount epd:module="B7">0</epd:amount>
<epd:amount epd:module="C1">0</epd:amount>
<epd:amount epd:module="C2">0.7198</epd:amount>
<epd:amount epd:module="C3">0.7428</epd:amount>
<epd:amount epd:module="C4">0</epd:amount>
<epd:amount epd:module="D">-100.1</epd:amount>
</common:other>
</LCIAResult>
</LCIAResults>
</processDataSet>